<?xml version="1.0"?>
<rdf:RDF xmlns="https://gitlab.atb-bremen.de/atb/pss-ontology/PSS-ontology-2#"
     xml:base="https://gitlab.atb-bremen.de/atb/pss-ontology/PSS-ontology-2"
     xmlns:dc="http://purl.org/dc/elements/1.1/"
     xmlns:bfo="http://purl.obolibrary.org/obo/bfo.owl#"
     xmlns:obo="http://purl.obolibrary.org/obo/"
     xmlns:owl="http://www.w3.org/2002/07/owl#"
     xmlns:rdf="http://www.w3.org/1999/02/22-rdf-syntax-ns#"
     xmlns:xml="http://www.w3.org/XML/1998/namespace"
     xmlns:xsd="http://www.w3.org/2001/XMLSchema#"
     xmlns:foaf="http://xmlns.com/foaf/0.1/"
     xmlns:obda="https://w3id.org/obda/vocabulary#"
     xmlns:rdfs="http://www.w3.org/2000/01/rdf-schema#"
     xmlns:terms="http://purl.org/dc/terms/"
     xmlns:oboInOwl="http://www.geneontology.org/formats/oboInOwl#"
     xmlns:PSS-ontology-2="http://www.semanticweb.org/atb/ontologies/2019/11/PSS-ontology-2#"
     xmlns:CommonCoreOntologies="http://www.ontologyrepository.com/CommonCoreOntologies/">
    <owl:Ontology rdf:about="https://gitlab.atb-bremen.de/atb/pss-ontology/PSS-ontology-2">
        <owl:versionIRI rdf:resource="https://gitlab.atb-bremen.de/atb/pss-ontology/PSS-ontology-2/0.2"/>
        <owl:imports rdf:resource="https://www.industrialontologies.org/core"/>
    </owl:Ontology>
    


    <!-- 
    ///////////////////////////////////////////////////////////////////////////////////////
    //
    // Annotation properties
    //
    ///////////////////////////////////////////////////////////////////////////////////////
     -->

    


    <!-- https://gitlab.atb-bremen.de/atb/pss-ontology/PSS-ontology-2#description -->

    <owl:AnnotationProperty rdf:about="https://gitlab.atb-bremen.de/atb/pss-ontology/PSS-ontology-2#description"/>
    


    <!-- 
    ///////////////////////////////////////////////////////////////////////////////////////
    //
    // Object Properties
    //
    ///////////////////////////////////////////////////////////////////////////////////////
     -->

    


    <!-- https://gitlab.atb-bremen.de/atb/pss-ontology/PSS-ontology-2#BusinessCustomer_owns_PSS -->

    <owl:ObjectProperty rdf:about="https://gitlab.atb-bremen.de/atb/pss-ontology/PSS-ontology-2#BusinessCustomer_owns_PSS"/>
    


    <!-- https://gitlab.atb-bremen.de/atb/pss-ontology/PSS-ontology-2#BusinessCustomer_owns_Product -->

    <owl:ObjectProperty rdf:about="https://gitlab.atb-bremen.de/atb/pss-ontology/PSS-ontology-2#BusinessCustomer_owns_Product"/>
    


    <!-- https://gitlab.atb-bremen.de/atb/pss-ontology/PSS-ontology-2#BusinessCustomer_owns_ServiceOffer -->

    <owl:ObjectProperty rdf:about="https://gitlab.atb-bremen.de/atb/pss-ontology/PSS-ontology-2#BusinessCustomer_owns_ServiceOffer"/>
    


    <!-- https://gitlab.atb-bremen.de/atb/pss-ontology/PSS-ontology-2#BusinessCustomer_provides_Feedback -->

    <owl:ObjectProperty rdf:about="https://gitlab.atb-bremen.de/atb/pss-ontology/PSS-ontology-2#BusinessCustomer_provides_Feedback"/>
    


    <!-- https://gitlab.atb-bremen.de/atb/pss-ontology/PSS-ontology-2#Company_uses_Feedback -->

    <owl:ObjectProperty rdf:about="https://gitlab.atb-bremen.de/atb/pss-ontology/PSS-ontology-2#Company_uses_Feedback"/>
    


    <!-- https://gitlab.atb-bremen.de/atb/pss-ontology/PSS-ontology-2#Company_uses_Guideline -->

    <owl:ObjectProperty rdf:about="https://gitlab.atb-bremen.de/atb/pss-ontology/PSS-ontology-2#Company_uses_Guideline"/>
    


    <!-- https://gitlab.atb-bremen.de/atb/pss-ontology/PSS-ontology-2#Company_uses_Indicator -->

    <owl:ObjectProperty rdf:about="https://gitlab.atb-bremen.de/atb/pss-ontology/PSS-ontology-2#Company_uses_Indicator"/>
    


    <!-- https://gitlab.atb-bremen.de/atb/pss-ontology/PSS-ontology-2#EmbeddedDataSourceComponent_generates_EmbeddedData -->

    <owl:ObjectProperty rdf:about="https://gitlab.atb-bremen.de/atb/pss-ontology/PSS-ontology-2#EmbeddedDataSourceComponent_generates_EmbeddedData"/>
    


    <!-- https://gitlab.atb-bremen.de/atb/pss-ontology/PSS-ontology-2#Employee_uses_Infrastructure -->

    <owl:ObjectProperty rdf:about="https://gitlab.atb-bremen.de/atb/pss-ontology/PSS-ontology-2#Employee_uses_Infrastructure"/>
    


    <!-- https://gitlab.atb-bremen.de/atb/pss-ontology/PSS-ontology-2#Feedback_refers_to_PSS -->

    <owl:ObjectProperty rdf:about="https://gitlab.atb-bremen.de/atb/pss-ontology/PSS-ontology-2#Feedback_refers_to_PSS"/>
    


    <!-- https://gitlab.atb-bremen.de/atb/pss-ontology/PSS-ontology-2#Feedback_refers_to_Product -->

    <owl:ObjectProperty rdf:about="https://gitlab.atb-bremen.de/atb/pss-ontology/PSS-ontology-2#Feedback_refers_to_Product"/>
    


    <!-- https://gitlab.atb-bremen.de/atb/pss-ontology/PSS-ontology-2#Feedback_refers_to_Service -->

    <owl:ObjectProperty rdf:about="https://gitlab.atb-bremen.de/atb/pss-ontology/PSS-ontology-2#Feedback_refers_to_Service"/>
    


    <!-- https://gitlab.atb-bremen.de/atb/pss-ontology/PSS-ontology-2#IndividualCustomer_owns_PSS -->

    <owl:ObjectProperty rdf:about="https://gitlab.atb-bremen.de/atb/pss-ontology/PSS-ontology-2#IndividualCustomer_owns_PSS"/>
    


    <!-- https://gitlab.atb-bremen.de/atb/pss-ontology/PSS-ontology-2#IndividualCustomer_owns_Product -->

    <owl:ObjectProperty rdf:about="https://gitlab.atb-bremen.de/atb/pss-ontology/PSS-ontology-2#IndividualCustomer_owns_Product"/>
    


    <!-- https://gitlab.atb-bremen.de/atb/pss-ontology/PSS-ontology-2#IndividualCustomer_owns_ServiceOffer -->

    <owl:ObjectProperty rdf:about="https://gitlab.atb-bremen.de/atb/pss-ontology/PSS-ontology-2#IndividualCustomer_owns_ServiceOffer"/>
    


    <!-- https://gitlab.atb-bremen.de/atb/pss-ontology/PSS-ontology-2#IndividualCustomer_provides_Feedback -->

    <owl:ObjectProperty rdf:about="https://gitlab.atb-bremen.de/atb/pss-ontology/PSS-ontology-2#IndividualCustomer_provides_Feedback"/>
    


    <!-- https://gitlab.atb-bremen.de/atb/pss-ontology/PSS-ontology-2#IndividualPerson_provides_Feedback -->

    <owl:ObjectProperty rdf:about="https://gitlab.atb-bremen.de/atb/pss-ontology/PSS-ontology-2#IndividualPerson_provides_Feedback"/>
    


    <!-- https://gitlab.atb-bremen.de/atb/pss-ontology/PSS-ontology-2#Lifecycle_implements_LifecycleModel -->

    <owl:ObjectProperty rdf:about="https://gitlab.atb-bremen.de/atb/pss-ontology/PSS-ontology-2#Lifecycle_implements_LifecycleModel"/>
    


    <!-- https://gitlab.atb-bremen.de/atb/pss-ontology/PSS-ontology-2#PSSCondition_refers_to_PSS -->

    <owl:ObjectProperty rdf:about="https://gitlab.atb-bremen.de/atb/pss-ontology/PSS-ontology-2#PSSCondition_refers_to_PSS"/>
    


    <!-- https://gitlab.atb-bremen.de/atb/pss-ontology/PSS-ontology-2#PSSProvider_supplies_PSS -->

    <owl:ObjectProperty rdf:about="https://gitlab.atb-bremen.de/atb/pss-ontology/PSS-ontology-2#PSSProvider_supplies_PSS"/>
    


    <!-- https://gitlab.atb-bremen.de/atb/pss-ontology/PSS-ontology-2#PSS_belongsTo_PSSProvider -->

    <owl:ObjectProperty rdf:about="https://gitlab.atb-bremen.de/atb/pss-ontology/PSS-ontology-2#PSS_belongsTo_PSSProvider">
        <rdfs:domain rdf:resource="https://gitlab.atb-bremen.de/atb/pss-ontology/PSS-ontology-2#PSS"/>
        <rdfs:range rdf:resource="https://gitlab.atb-bremen.de/atb/pss-ontology/PSS-ontology-2#PSS_Provider"/>
    </owl:ObjectProperty>
    


    <!-- https://gitlab.atb-bremen.de/atb/pss-ontology/PSS-ontology-2#PSS_exists_in_PSSLifecycle -->

    <owl:ObjectProperty rdf:about="https://gitlab.atb-bremen.de/atb/pss-ontology/PSS-ontology-2#PSS_exists_in_PSSLifecycle"/>
    


    <!-- https://gitlab.atb-bremen.de/atb/pss-ontology/PSS-ontology-2#PSS_has_PSSFeature -->

    <owl:ObjectProperty rdf:about="https://gitlab.atb-bremen.de/atb/pss-ontology/PSS-ontology-2#PSS_has_PSSFeature"/>
    


    <!-- https://gitlab.atb-bremen.de/atb/pss-ontology/PSS-ontology-2#PSS_has_PSSLifecycleModel -->

    <owl:ObjectProperty rdf:about="https://gitlab.atb-bremen.de/atb/pss-ontology/PSS-ontology-2#PSS_has_PSSLifecycleModel"/>
    


    <!-- https://gitlab.atb-bremen.de/atb/pss-ontology/PSS-ontology-2#PSS_has_PSSRole -->

    <owl:ObjectProperty rdf:about="https://gitlab.atb-bremen.de/atb/pss-ontology/PSS-ontology-2#PSS_has_PSSRole"/>
    


    <!-- https://gitlab.atb-bremen.de/atb/pss-ontology/PSS-ontology-2#PSS_implements_BusinessModel -->

    <owl:ObjectProperty rdf:about="https://gitlab.atb-bremen.de/atb/pss-ontology/PSS-ontology-2#PSS_implements_BusinessModel"/>
    


    <!-- https://gitlab.atb-bremen.de/atb/pss-ontology/PSS-ontology-2#PSS_is_composed_of_Product -->

    <owl:ObjectProperty rdf:about="https://gitlab.atb-bremen.de/atb/pss-ontology/PSS-ontology-2#PSS_is_composed_of_Product"/>
    


    <!-- https://gitlab.atb-bremen.de/atb/pss-ontology/PSS-ontology-2#PSS_is_composed_of_ServiceOffer -->

    <owl:ObjectProperty rdf:about="https://gitlab.atb-bremen.de/atb/pss-ontology/PSS-ontology-2#PSS_is_composed_of_ServiceOffer"/>
    


    <!-- https://gitlab.atb-bremen.de/atb/pss-ontology/PSS-ontology-2#PSS_uses_Resource -->

    <owl:ObjectProperty rdf:about="https://gitlab.atb-bremen.de/atb/pss-ontology/PSS-ontology-2#PSS_uses_Resource"/>
    


    <!-- https://gitlab.atb-bremen.de/atb/pss-ontology/PSS-ontology-2#Process_implements_ProcessDefinition -->

    <owl:ObjectProperty rdf:about="https://gitlab.atb-bremen.de/atb/pss-ontology/PSS-ontology-2#Process_implements_ProcessDefinition"/>
    


    <!-- https://gitlab.atb-bremen.de/atb/pss-ontology/PSS-ontology-2#ProductExtensionServiceOffer_extends_Product -->

    <owl:ObjectProperty rdf:about="https://gitlab.atb-bremen.de/atb/pss-ontology/PSS-ontology-2#ProductExtensionServiceOffer_extends_Product"/>
    


    <!-- https://gitlab.atb-bremen.de/atb/pss-ontology/PSS-ontology-2#ProductExtensionServiceOffer_uses_ProductData -->

    <owl:ObjectProperty rdf:about="https://gitlab.atb-bremen.de/atb/pss-ontology/PSS-ontology-2#ProductExtensionServiceOffer_uses_ProductData"/>
    


    <!-- https://gitlab.atb-bremen.de/atb/pss-ontology/PSS-ontology-2#ProductIntegratedSet_is_composed_of_Products -->

    <owl:ObjectProperty rdf:about="https://gitlab.atb-bremen.de/atb/pss-ontology/PSS-ontology-2#ProductIntegratedSet_is_composed_of_Products"/>
    


    <!-- https://gitlab.atb-bremen.de/atb/pss-ontology/PSS-ontology-2#ProductProvider_supplies_Product -->

    <owl:ObjectProperty rdf:about="https://gitlab.atb-bremen.de/atb/pss-ontology/PSS-ontology-2#ProductProvider_supplies_Product"/>
    


    <!-- https://gitlab.atb-bremen.de/atb/pss-ontology/PSS-ontology-2#ProductProvider_supplies_ProductComponent -->

    <owl:ObjectProperty rdf:about="https://gitlab.atb-bremen.de/atb/pss-ontology/PSS-ontology-2#ProductProvider_supplies_ProductComponent"/>
    


    <!-- https://gitlab.atb-bremen.de/atb/pss-ontology/PSS-ontology-2#Product_exists_in_ProductLifecycle -->

    <owl:ObjectProperty rdf:about="https://gitlab.atb-bremen.de/atb/pss-ontology/PSS-ontology-2#Product_exists_in_ProductLifecycle"/>
    


    <!-- https://gitlab.atb-bremen.de/atb/pss-ontology/PSS-ontology-2#Product_has_ProductFeature -->

    <owl:ObjectProperty rdf:about="https://gitlab.atb-bremen.de/atb/pss-ontology/PSS-ontology-2#Product_has_ProductFeature"/>
    


    <!-- https://gitlab.atb-bremen.de/atb/pss-ontology/PSS-ontology-2#Product_has_ProductLifecycleModel -->

    <owl:ObjectProperty rdf:about="https://gitlab.atb-bremen.de/atb/pss-ontology/PSS-ontology-2#Product_has_ProductLifecycleModel"/>
    


    <!-- https://gitlab.atb-bremen.de/atb/pss-ontology/PSS-ontology-2#Product_has_ProductRole -->

    <owl:ObjectProperty rdf:about="https://gitlab.atb-bremen.de/atb/pss-ontology/PSS-ontology-2#Product_has_ProductRole"/>
    


    <!-- https://gitlab.atb-bremen.de/atb/pss-ontology/PSS-ontology-2#Product_is_composed_of_ProductComponent -->

    <owl:ObjectProperty rdf:about="https://gitlab.atb-bremen.de/atb/pss-ontology/PSS-ontology-2#Product_is_composed_of_ProductComponent"/>
    


    <!-- https://gitlab.atb-bremen.de/atb/pss-ontology/PSS-ontology-2#ServiceComponent_implements_ServiceOfferComponent -->

    <owl:ObjectProperty rdf:about="https://gitlab.atb-bremen.de/atb/pss-ontology/PSS-ontology-2#ServiceComponent_implements_ServiceOfferComponent"/>
    


    <!-- https://gitlab.atb-bremen.de/atb/pss-ontology/PSS-ontology-2#ServiceOfferIntegratedSet_is_composed_of_ServiceOffers -->

    <owl:ObjectProperty rdf:about="https://gitlab.atb-bremen.de/atb/pss-ontology/PSS-ontology-2#ServiceOfferIntegratedSet_is_composed_of_ServiceOffers"/>
    


    <!-- https://gitlab.atb-bremen.de/atb/pss-ontology/PSS-ontology-2#ServiceOffer_has_ServiceLifecycleModel -->

    <owl:ObjectProperty rdf:about="https://gitlab.atb-bremen.de/atb/pss-ontology/PSS-ontology-2#ServiceOffer_has_ServiceLifecycleModel"/>
    


    <!-- https://gitlab.atb-bremen.de/atb/pss-ontology/PSS-ontology-2#ServiceOffer_has_ServiceOfferFeature -->

    <owl:ObjectProperty rdf:about="https://gitlab.atb-bremen.de/atb/pss-ontology/PSS-ontology-2#ServiceOffer_has_ServiceOfferFeature"/>
    


    <!-- https://gitlab.atb-bremen.de/atb/pss-ontology/PSS-ontology-2#ServiceOffer_is_part_of_PSS -->

    <owl:ObjectProperty rdf:about="https://gitlab.atb-bremen.de/atb/pss-ontology/PSS-ontology-2#ServiceOffer_is_part_of_PSS"/>
    


    <!-- https://gitlab.atb-bremen.de/atb/pss-ontology/PSS-ontology-2#ServiceProvider_supplies_Service -->

    <owl:ObjectProperty rdf:about="https://gitlab.atb-bremen.de/atb/pss-ontology/PSS-ontology-2#ServiceProvider_supplies_Service"/>
    


    <!-- https://gitlab.atb-bremen.de/atb/pss-ontology/PSS-ontology-2#Service_exists_in_ServiceLifecycleModel -->

    <owl:ObjectProperty rdf:about="https://gitlab.atb-bremen.de/atb/pss-ontology/PSS-ontology-2#Service_exists_in_ServiceLifecycleModel"/>
    


    <!-- https://gitlab.atb-bremen.de/atb/pss-ontology/PSS-ontology-2#Service_generates_ServiceData -->

    <owl:ObjectProperty rdf:about="https://gitlab.atb-bremen.de/atb/pss-ontology/PSS-ontology-2#Service_generates_ServiceData"/>
    


    <!-- https://gitlab.atb-bremen.de/atb/pss-ontology/PSS-ontology-2#Service_implements_PSS -->

    <owl:ObjectProperty rdf:about="https://gitlab.atb-bremen.de/atb/pss-ontology/PSS-ontology-2#Service_implements_PSS"/>
    


    <!-- https://gitlab.atb-bremen.de/atb/pss-ontology/PSS-ontology-2#Service_implements_ServiceOffer -->

    <owl:ObjectProperty rdf:about="https://gitlab.atb-bremen.de/atb/pss-ontology/PSS-ontology-2#Service_implements_ServiceOffer"/>
    


    <!-- https://gitlab.atb-bremen.de/atb/pss-ontology/PSS-ontology-2#Service_is_composed_of_ServiceComponent -->

    <owl:ObjectProperty rdf:about="https://gitlab.atb-bremen.de/atb/pss-ontology/PSS-ontology-2#Service_is_composed_of_ServiceComponent"/>
    


    <!-- https://gitlab.atb-bremen.de/atb/pss-ontology/PSS-ontology-2#Service_uses_ProductData -->

    <owl:ObjectProperty rdf:about="https://gitlab.atb-bremen.de/atb/pss-ontology/PSS-ontology-2#Service_uses_ProductData"/>
    


    <!-- https://gitlab.atb-bremen.de/atb/pss-ontology/PSS-ontology-2#Service_uses_ServiceData -->

    <owl:ObjectProperty rdf:about="https://gitlab.atb-bremen.de/atb/pss-ontology/PSS-ontology-2#Service_uses_ServiceData"/>
    


    <!-- https://gitlab.atb-bremen.de/atb/pss-ontology/PSS-ontology-2#Stakeholder_defines_Requirements -->

    <owl:ObjectProperty rdf:about="https://gitlab.atb-bremen.de/atb/pss-ontology/PSS-ontology-2#Stakeholder_defines_Requirements"/>
    


    <!-- https://gitlab.atb-bremen.de/atb/pss-ontology/PSS-ontology-2#Stakeholder_provides_Feedback -->

    <owl:ObjectProperty rdf:about="https://gitlab.atb-bremen.de/atb/pss-ontology/PSS-ontology-2#Stakeholder_provides_Feedback"/>
    


    <!-- 
    ///////////////////////////////////////////////////////////////////////////////////////
    //
    // Classes
    //
    ///////////////////////////////////////////////////////////////////////////////////////
     -->

    


    <!-- http://purl.obolibrary.org/obo/BFO_0000002 -->

    <owl:Class rdf:about="http://purl.obolibrary.org/obo/BFO_0000002"/>
    


    <!-- http://purl.obolibrary.org/obo/BFO_0000015 -->

    <owl:Class rdf:about="http://purl.obolibrary.org/obo/BFO_0000015"/>
    


    <!-- http://purl.obolibrary.org/obo/BFO_0000017 -->

    <owl:Class rdf:about="http://purl.obolibrary.org/obo/BFO_0000017"/>
    


    <!-- http://purl.obolibrary.org/obo/BFO_0000020 -->

    <owl:Class rdf:about="http://purl.obolibrary.org/obo/BFO_0000020"/>
    


    <!-- http://purl.obolibrary.org/obo/BFO_0000023 -->

    <owl:Class rdf:about="http://purl.obolibrary.org/obo/BFO_0000023"/>
    


    <!-- http://purl.obolibrary.org/obo/BFO_0000031 -->

    <owl:Class rdf:about="http://purl.obolibrary.org/obo/BFO_0000031"/>
    


    <!-- http://purl.obolibrary.org/obo/BFO_0000040 -->

    <owl:Class rdf:about="http://purl.obolibrary.org/obo/BFO_0000040"/>
    


    <!-- http://purl.obolibrary.org/obo/BFO_0000141 -->

    <owl:Class rdf:about="http://purl.obolibrary.org/obo/BFO_0000141"/>
    


    <!-- https://gitlab.atb-bremen.de/atb/pss-ontology/PSS-ontology-2#Benefit -->

    <owl:Class rdf:about="https://gitlab.atb-bremen.de/atb/pss-ontology/PSS-ontology-2#Benefit">
        <rdfs:subClassOf rdf:resource="https://gitlab.atb-bremen.de/atb/pss-ontology/PSS-ontology-2#Indicator"/>
        <obo:IAO_0000115>Benefit is an indicator that depicts a positive value (e.g. financial, satisfaction, assistance, etc.)  a stakeholder (e.g. a customer) receives back as a result of the offered PSS.</obo:IAO_0000115>
        <dc:contributor>ATB - EPFL</dc:contributor>
        <rdfs:comment>Examples could be e.g.
cost reduction, eco friendliness, performance improvement, risk reduction.</rdfs:comment>
        <rdfs:label>benefit</rdfs:label>
    </owl:Class>
    


    <!-- https://gitlab.atb-bremen.de/atb/pss-ontology/PSS-ontology-2#BusinessProcess -->

    <owl:Class rdf:about="https://gitlab.atb-bremen.de/atb/pss-ontology/PSS-ontology-2#BusinessProcess">
        <rdfs:subClassOf rdf:resource="http://purl.obolibrary.org/obo/BFO_0000015"/>
        <obo:IAO_0000115>A business process is a planned process that realizes a function of an organization (company/enterprise).</obo:IAO_0000115>
        <dc:contributor>ATB - EPFL</dc:contributor>
        <rdfs:label>Business Process</rdfs:label>
    </owl:Class>
    


    <!-- https://gitlab.atb-bremen.de/atb/pss-ontology/PSS-ontology-2#BusinessResource -->

    <owl:Class rdf:about="https://gitlab.atb-bremen.de/atb/pss-ontology/PSS-ontology-2#BusinessResource">
        <rdfs:subClassOf rdf:resource="https://gitlab.atb-bremen.de/atb/pss-ontology/PSS-ontology-2#Resource"/>
        <obo:IAO_0000115>Business resource =def. continuant that bears a business resource role.</obo:IAO_0000115>
        <dc:contributor>ATB - EPFL</dc:contributor>
        <rdfs:label>Business Resource</rdfs:label>
    </owl:Class>
    


    <!-- https://gitlab.atb-bremen.de/atb/pss-ontology/PSS-ontology-2#BusinessResourceRole -->

    <owl:Class rdf:about="https://gitlab.atb-bremen.de/atb/pss-ontology/PSS-ontology-2#BusinessResourceRole">
        <rdfs:subClassOf rdf:resource="http://purl.obolibrary.org/obo/BFO_0000023"/>
        <obo:IAO_0000115>business resource role is a role that inheres in an independent continuant where that continuant bears a disposition that, if realized, is realized in a business enterprise process</obo:IAO_0000115>
        <dc:contributor>ATB - EPFL</dc:contributor>
        <rdfs:label>Business Resource Role</rdfs:label>
    </owl:Class>
    


    <!-- https://gitlab.atb-bremen.de/atb/pss-ontology/PSS-ontology-2#Business_Customer -->

    <owl:Class rdf:about="https://gitlab.atb-bremen.de/atb/pss-ontology/PSS-ontology-2#Business_Customer">
        <rdfs:subClassOf rdf:resource="https://gitlab.atb-bremen.de/atb/pss-ontology/PSS-ontology-2#Company"/>
        <obo:IAO_0000115>Business Customer is a Company that buys and uses the products, services or PSS. It is the (group/company) customer of the PSS, using the PSS for their own business.</obo:IAO_0000115>
        <dc:contributor>ATB - EPFL</dc:contributor>
        <rdfs:label>Business Customer</rdfs:label>
    </owl:Class>
    


    <!-- https://gitlab.atb-bremen.de/atb/pss-ontology/PSS-ontology-2#Business_Model -->

    <owl:Class rdf:about="https://gitlab.atb-bremen.de/atb/pss-ontology/PSS-ontology-2#Business_Model">
        <rdfs:subClassOf rdf:resource="http://purl.obolibrary.org/obo/BFO_0000020"/>
        <obo:IAO_0000115>Business Model is a description of a plan and implementation of the plan, aiming the successful operation of a business.</obo:IAO_0000115>
        <dc:contributor>ATB - EPFL</dc:contributor>
        <rdfs:comment>This is an interface class to other ontologies.</rdfs:comment>
        <rdfs:label>Business Model</rdfs:label>
    </owl:Class>
    


    <!-- https://gitlab.atb-bremen.de/atb/pss-ontology/PSS-ontology-2#Company -->

    <owl:Class rdf:about="https://gitlab.atb-bremen.de/atb/pss-ontology/PSS-ontology-2#Company">
        <rdfs:subClassOf rdf:resource="https://gitlab.atb-bremen.de/atb/pss-ontology/PSS-ontology-2#Stakeholder/Actor"/>
        <obo:IAO_0000115>Company is a Stakeholder that can be one or more individuals forming a legal entity (corporate body).</obo:IAO_0000115>
        <dc:contributor>ATB - EPFL</dc:contributor>
        <rdfs:label>Company</rdfs:label>
    </owl:Class>
    


    <!-- https://gitlab.atb-bremen.de/atb/pss-ontology/PSS-ontology-2#Data -->

    <owl:Class rdf:about="https://gitlab.atb-bremen.de/atb/pss-ontology/PSS-ontology-2#Data">
        <rdfs:subClassOf rdf:resource="https://gitlab.atb-bremen.de/atb/pss-ontology/PSS-ontology-2#Resource"/>
        <obo:IAO_0000115>PSS Source-Data is a Resource that refers to the digitalised information coming as input from the product or the service, specifically for the scope of PSS.</obo:IAO_0000115>
        <dc:contributor>ATB - EPFL</dc:contributor>
        <rdfs:label>PSS Source-Data</rdfs:label>
    </owl:Class>
    


    <!-- https://gitlab.atb-bremen.de/atb/pss-ontology/PSS-ontology-2#Embedded_Data -->

    <owl:Class rdf:about="https://gitlab.atb-bremen.de/atb/pss-ontology/PSS-ontology-2#Embedded_Data">
        <rdfs:subClassOf rdf:resource="https://gitlab.atb-bremen.de/atb/pss-ontology/PSS-ontology-2#Product_Data"/>
        <obo:IAO_0000115>Embedded Data are Product Data generated from embedded data-source components (e.g. sensors).</obo:IAO_0000115>
        <dc:contributor>ATB - EPFL</dc:contributor>
        <rdfs:label>Embedded Data</rdfs:label>
    </owl:Class>
    


    <!-- https://gitlab.atb-bremen.de/atb/pss-ontology/PSS-ontology-2#Embedded_Data_Source_Component -->

    <owl:Class rdf:about="https://gitlab.atb-bremen.de/atb/pss-ontology/PSS-ontology-2#Embedded_Data_Source_Component">
        <rdfs:subClassOf rdf:resource="https://gitlab.atb-bremen.de/atb/pss-ontology/PSS-ontology-2#Product_Component"/>
        <obo:IAO_0000115>Embedded Data-Source Component is a Product Component that refers to product-embedded information devices / parts (e.g. sensors), which allows for (additional) services to be offered for the product.</obo:IAO_0000115>
        <dc:contributor>ATB - EPFL</dc:contributor>
        <rdfs:label>Embedded Data-Source Component</rdfs:label>
    </owl:Class>
    


    <!-- https://gitlab.atb-bremen.de/atb/pss-ontology/PSS-ontology-2#Employee -->

    <owl:Class rdf:about="https://gitlab.atb-bremen.de/atb/pss-ontology/PSS-ontology-2#Employee">
        <rdfs:subClassOf rdf:resource="https://gitlab.atb-bremen.de/atb/pss-ontology/PSS-ontology-2#Individual_Person"/>
        <obo:IAO_0000115>Employee is an Individual Person that works in a Company (PSS-related company).</obo:IAO_0000115>
        <dc:contributor>ATB - EPFL</dc:contributor>
        <rdfs:label>Employee</rdfs:label>
    </owl:Class>
    


    <!-- https://gitlab.atb-bremen.de/atb/pss-ontology/PSS-ontology-2#Feature -->

    <owl:Class rdf:about="https://gitlab.atb-bremen.de/atb/pss-ontology/PSS-ontology-2#Feature">
        <rdfs:subClassOf rdf:resource="https://gitlab.atb-bremen.de/atb/pss-ontology/PSS-ontology-2#Information"/>
        <obo:IAO_0000115>Feature is PSS Information that describes the characteristics of a product, service, or PSS.</obo:IAO_0000115>
        <dc:contributor>ATB - EPFL</dc:contributor>
    </owl:Class>
    


    <!-- https://gitlab.atb-bremen.de/atb/pss-ontology/PSS-ontology-2#Feedback -->

    <owl:Class rdf:about="https://gitlab.atb-bremen.de/atb/pss-ontology/PSS-ontology-2#Feedback">
        <rdfs:subClassOf rdf:resource="https://gitlab.atb-bremen.de/atb/pss-ontology/PSS-ontology-2#Information"/>
        <obo:IAO_0000115>Feedback is PSS Information that represents any opinion on PSS, product or service (e.g. comments on social media, opinion expression in online questionnaires, etc.), coming from the Stakeholders (e.g., Business or Individual Customers).</obo:IAO_0000115>
        <dc:contributor>ATB - EPFL</dc:contributor>
        <rdfs:label>Feedback</rdfs:label>
    </owl:Class>
    


    <!-- https://gitlab.atb-bremen.de/atb/pss-ontology/PSS-ontology-2#Firmware -->

    <owl:Class rdf:about="https://gitlab.atb-bremen.de/atb/pss-ontology/PSS-ontology-2#Firmware">
        <rdfs:subClassOf rdf:resource="https://gitlab.atb-bremen.de/atb/pss-ontology/PSS-ontology-2#Product_Component"/>
        <obo:IAO_0000115>Firmware is a Product Component which is software, i.e. control software of a machine that exists only in combination with specific hardware product.</obo:IAO_0000115>
        <dc:contributor>ATB - EPFL</dc:contributor>
    </owl:Class>
    


    <!-- https://gitlab.atb-bremen.de/atb/pss-ontology/PSS-ontology-2#Guideline -->

    <owl:Class rdf:about="https://gitlab.atb-bremen.de/atb/pss-ontology/PSS-ontology-2#Guideline">
        <rdfs:subClassOf rdf:resource="https://gitlab.atb-bremen.de/atb/pss-ontology/PSS-ontology-2#Information"/>
        <obo:IAO_0000115>Guideline is PSS Information referring to a statement describing a course of action aiming to reach a specific goal for the design, development or use of a PSS.</obo:IAO_0000115>
        <dc:contributor>ATB - EPFL</dc:contributor>
        <rdfs:label>Guideline</rdfs:label>
    </owl:Class>
    


    <!-- https://gitlab.atb-bremen.de/atb/pss-ontology/PSS-ontology-2#Hardware_Infrastructure -->

    <owl:Class rdf:about="https://gitlab.atb-bremen.de/atb/pss-ontology/PSS-ontology-2#Hardware_Infrastructure">
        <rdfs:subClassOf rdf:resource="https://gitlab.atb-bremen.de/atb/pss-ontology/PSS-ontology-2#Infrastructure"/>
        <obo:IAO_0000115>Hardware Infrastructure is an Infrastructure that refers to the physical networks (resources) necessary for the design, development, delivery and operation of the PSS.</obo:IAO_0000115>
        <dc:contributor>ATB - EPFL</dc:contributor>
        <rdfs:label>Hardware Infrastucture</rdfs:label>
    </owl:Class>
    


    <!-- https://gitlab.atb-bremen.de/atb/pss-ontology/PSS-ontology-2#Indicator -->

    <owl:Class rdf:about="https://gitlab.atb-bremen.de/atb/pss-ontology/PSS-ontology-2#Indicator">
        <rdfs:subClassOf rdf:resource="https://gitlab.atb-bremen.de/atb/pss-ontology/PSS-ontology-2#Information"/>
        <obo:IAO_0000115>Indicator is PSS Information used to measure/evaluate any aspect within the scope of PSS, namely a process, a PSS, a product, a service, etc.</obo:IAO_0000115>
        <dc:contributor>ATB - EPFL</dc:contributor>
        <rdfs:label>Indicator</rdfs:label>
    </owl:Class>
    


    <!-- https://gitlab.atb-bremen.de/atb/pss-ontology/PSS-ontology-2#Individual_Customer -->

    <owl:Class rdf:about="https://gitlab.atb-bremen.de/atb/pss-ontology/PSS-ontology-2#Individual_Customer">
        <rdfs:subClassOf rdf:resource="https://gitlab.atb-bremen.de/atb/pss-ontology/PSS-ontology-2#Individual_Person"/>
        <obo:IAO_0000115>Individual Customer (Consumer) is an Individual Person that buys or consumes (consumer) any product/service in the PSS.</obo:IAO_0000115>
        <dc:contributor>ATB - EPFL</dc:contributor>
        <rdfs:label>Individual Customer (Consumer)</rdfs:label>
    </owl:Class>
    


    <!-- https://gitlab.atb-bremen.de/atb/pss-ontology/PSS-ontology-2#Individual_Person -->

    <owl:Class rdf:about="https://gitlab.atb-bremen.de/atb/pss-ontology/PSS-ontology-2#Individual_Person">
        <rdfs:subClassOf rdf:resource="https://gitlab.atb-bremen.de/atb/pss-ontology/PSS-ontology-2#Stakeholder/Actor"/>
        <obo:IAO_0000115>Individual Person is a Stakeholder indicating a separate person who is not legal entity (i.e. not legally considered a corporate group, as for example a company).</obo:IAO_0000115>
        <dc:contributor>ATB - EPFL</dc:contributor>
        <rdfs:label>Individual Person</rdfs:label>
    </owl:Class>
    


    <!-- https://gitlab.atb-bremen.de/atb/pss-ontology/PSS-ontology-2#Information -->

    <owl:Class rdf:about="https://gitlab.atb-bremen.de/atb/pss-ontology/PSS-ontology-2#Information">
        <rdfs:subClassOf rdf:resource="https://gitlab.atb-bremen.de/atb/pss-ontology/PSS-ontology-2#Resource"/>
        <obo:IAO_0000115>PSS Information is a Resource, immaterial, describing aspects affecting PSS, and referring to all the (processed) data that one can acquire knowledge from, or further process.</obo:IAO_0000115>
        <dc:contributor>ATB - EPFL</dc:contributor>
        <rdfs:comment>Name to be changed to Immaterial Resources?</rdfs:comment>
        <rdfs:label>PSS Information</rdfs:label>
    </owl:Class>
    


    <!-- https://gitlab.atb-bremen.de/atb/pss-ontology/PSS-ontology-2#Infrastructure -->

    <owl:Class rdf:about="https://gitlab.atb-bremen.de/atb/pss-ontology/PSS-ontology-2#Infrastructure">
        <rdfs:subClassOf rdf:resource="https://gitlab.atb-bremen.de/atb/pss-ontology/PSS-ontology-2#Resource"/>
        <obo:IAO_0000115>Infrastructure is a Resource describing the facilities (physical e.g. buildings or machines, and organisational e.g. computer networks or software applications) used to assist in development and delivering of the PSS.</obo:IAO_0000115>
        <obo:IAO_0000118>Infrastructure is a Material Resource including the physical (e.g. buildings or machines, computers), and organisational (e.g. communication networks) means used to assist in development and delivering of the Product and Services.</obo:IAO_0000118>
        <dc:contributor>ATB - EPFL</dc:contributor>
        <rdfs:comment>It may serve as an interface class for merging with other ontologies.</rdfs:comment>
        <rdfs:label>Infrastructure</rdfs:label>
    </owl:Class>
    


    <!-- https://gitlab.atb-bremen.de/atb/pss-ontology/PSS-ontology-2#KPI -->

    <owl:Class rdf:about="https://gitlab.atb-bremen.de/atb/pss-ontology/PSS-ontology-2#KPI">
        <rdfs:subClassOf rdf:resource="https://gitlab.atb-bremen.de/atb/pss-ontology/PSS-ontology-2#Indicator"/>
        <obo:IAO_0000115>Key Performance Indicator (KPI) is an Indicator referring to (a set of) measurement(s) that evaluates the performance (or success) of a PSS (concept), and is business relevant.</obo:IAO_0000115>
        <dc:contributor>ATB - EPFL</dc:contributor>
        <rdfs:comment>Various types of KPIs can be defined: manufacturing KPI, environmental KPI etc. 
This is an interface class to other ontologies</rdfs:comment>
    </owl:Class>
    


    <!-- https://gitlab.atb-bremen.de/atb/pss-ontology/PSS-ontology-2#Lifecycle -->

    <owl:Class rdf:about="https://gitlab.atb-bremen.de/atb/pss-ontology/PSS-ontology-2#Lifecycle">
        <rdfs:subClassOf rdf:resource="http://purl.obolibrary.org/obo/BFO_0000015"/>
        <obo:IAO_0000115>Lifecycle is a set of Processes the PSS, a product or a service uses for its activities from the idea conceptualisation to its end-of-life. It refers to the Lifecycle Model entity in conjunction with time.</obo:IAO_0000115>
        <dc:contributor>ATB - EPFL</dc:contributor>
        <rdfs:comment>This is an interface class to other ontologies.</rdfs:comment>
        <rdfs:label>Lifecycle</rdfs:label>
    </owl:Class>
    


    <!-- https://gitlab.atb-bremen.de/atb/pss-ontology/PSS-ontology-2#Lifecycle_Model -->

    <owl:Class rdf:about="https://gitlab.atb-bremen.de/atb/pss-ontology/PSS-ontology-2#Lifecycle_Model">
        <rdfs:subClassOf rdf:resource="http://purl.obolibrary.org/obo/BFO_0000017"/>
        <obo:IAO_0000115>Lifecycle Model is a (set of) Process Definition(s) which includes different activities in the life of PSS, product, service etc. from the idea conceptualisation to its end-of life (beginning-of -life, middle-of-life, end-of-life).</obo:IAO_0000115>
        <dc:contributor>ATB - EPFL</dc:contributor>
        <rdfs:comment>This is an interface class to other ontologies.</rdfs:comment>
        <rdfs:label>Lifecycle Model</rdfs:label>
    </owl:Class>
    


    <!-- https://gitlab.atb-bremen.de/atb/pss-ontology/PSS-ontology-2#ManufacturingEnterpriseProcess -->

    <owl:Class rdf:about="https://gitlab.atb-bremen.de/atb/pss-ontology/PSS-ontology-2#ManufacturingEnterpriseProcess">
        <rdfs:subClassOf rdf:resource="http://purl.obolibrary.org/obo/BFO_0000015"/>
        <obo:IAO_0000115>Manufacturing enterprise process=def. planned process that has agent some manufacturing enterprise, where the agent realizes the planned processes of the enterprise.</obo:IAO_0000115>
        <dc:contributor>ATB - EPFL</dc:contributor>
        <rdfs:label>Manufacturing Enterprise Process</rdfs:label>
    </owl:Class>
    


    <!-- https://gitlab.atb-bremen.de/atb/pss-ontology/PSS-ontology-2#ManufacturingResource -->

    <owl:Class rdf:about="https://gitlab.atb-bremen.de/atb/pss-ontology/PSS-ontology-2#ManufacturingResource">
        <rdfs:subClassOf rdf:resource="https://gitlab.atb-bremen.de/atb/pss-ontology/PSS-ontology-2#Resource"/>
        <obo:IAO_0000115>IOF: Manufacturing resource =def. continuant that bears a manufacturing resource role.</obo:IAO_0000115>
        <dc:contributor>ATB - EPFL</dc:contributor>
        <rdfs:label>Manufacturing Resource</rdfs:label>
    </owl:Class>
    


    <!-- https://gitlab.atb-bremen.de/atb/pss-ontology/PSS-ontology-2#ManufacturingResourceRole -->

    <owl:Class rdf:about="https://gitlab.atb-bremen.de/atb/pss-ontology/PSS-ontology-2#ManufacturingResourceRole">
        <rdfs:subClassOf rdf:resource="http://purl.obolibrary.org/obo/BFO_0000023"/>
        <obo:IAO_0000115>Is a role that inheres in an independent continuant where that continuant bears a disposition that, if realized, is realized in a manufacturing enterprise process</obo:IAO_0000115>
        <rdfs:label>Manufacturing Resource Role</rdfs:label>
    </owl:Class>
    


    <!-- https://gitlab.atb-bremen.de/atb/pss-ontology/PSS-ontology-2#Material_Object -->

    <owl:Class rdf:about="https://gitlab.atb-bremen.de/atb/pss-ontology/PSS-ontology-2#Material_Object">
        <rdfs:subClassOf rdf:resource="http://purl.obolibrary.org/obo/BFO_0000002"/>
        <obo:IAO_0000115>Material Object is a group describing manufactured physical/material entities.</obo:IAO_0000115>
        <dc:contributor>ATB - EPFL</dc:contributor>
        <rdfs:label>Material Object</rdfs:label>
    </owl:Class>
    


    <!-- https://gitlab.atb-bremen.de/atb/pss-ontology/PSS-ontology-2#PSS -->

    <owl:Class rdf:about="https://gitlab.atb-bremen.de/atb/pss-ontology/PSS-ontology-2#PSS">
        <rdfs:subClassOf rdf:resource="https://gitlab.atb-bremen.de/atb/pss-ontology/PSS-ontology-2#System"/>
        <obo:IAO_0000115>Product Service System (PSS) is a System that aims to satisfy a need of the market (e.g. to be sold in order to provide profit and support customers by covering their needs), to be competitive, and jointly fulfil customer’s needs [3]. It must include products and services, and may include stakeholders and infrastructure (software or hardware).</obo:IAO_0000115>
        <obo:IAO_0000118>PSS is a system which includes at least one product and at least one service, related to this product, and may include stakeholders and infrastructure and which bears PSS Role.</obo:IAO_0000118>
        <obo:IAO_0000118>PSS is a system which includes at least one product and at least one service, related to this product, and which bears PSS Role.
PSS role is a role that borne by set of at least an entity that is the specified output of a product production process and at least an entity that is the specified output of a service development process</obo:IAO_0000118>
        <obo:IAO_0000119>Resources:

3. Mont, Oksana K. &quot;Clarifying the concept of product–service system.&quot; Journal of cleaner production 10.3 (2002): 237-245.</obo:IAO_0000119>
        <dc:contributor>ATB - EPFL</dc:contributor>
        <CommonCoreOntologies:acronym>PSS</CommonCoreOntologies:acronym>
        <rdfs:comment>This is an interface class to other ontologies.</rdfs:comment>
        <rdfs:label>PSS</rdfs:label>
    </owl:Class>
    


    <!-- https://gitlab.atb-bremen.de/atb/pss-ontology/PSS-ontology-2#PSS-Development_Condition -->

    <owl:Class rdf:about="https://gitlab.atb-bremen.de/atb/pss-ontology/PSS-ontology-2#PSS-Development_Condition">
        <rdfs:subClassOf rdf:resource="https://gitlab.atb-bremen.de/atb/pss-ontology/PSS-ontology-2#PSS_Condition"/>
        <obo:IAO_0000115>PSS-Development Condition is a PSS Condition which describes the situation under which the PSS is being developed (e.g. cultural characteristics of the development teams, corporate orientation preferences, etc.)</obo:IAO_0000115>
        <dc:contributor>ATB - EPFL</dc:contributor>
        <rdfs:comment>It may serve as an interface class for merging with other ontologies (e.g. in DIVERSITY to user-centric ontology [7]).</rdfs:comment>
        <rdfs:label>PSS-Development Condition</rdfs:label>
    </owl:Class>
    


    <!-- https://gitlab.atb-bremen.de/atb/pss-ontology/PSS-ontology-2#PSS-Use_Condition -->

    <owl:Class rdf:about="https://gitlab.atb-bremen.de/atb/pss-ontology/PSS-ontology-2#PSS-Use_Condition">
        <rdfs:subClassOf rdf:resource="https://gitlab.atb-bremen.de/atb/pss-ontology/PSS-ontology-2#PSS_Condition"/>
        <obo:IAO_0000115>PSS-Use Condition is a PSS Condition which describes the situation under which the PSS is being used (e.g. environment aspects, cultural aspect, geographical location, etc.).</obo:IAO_0000115>
        <dc:contributor>ATB - EPFL</dc:contributor>
        <rdfs:comment>It may serve as an interface class for merging with other ontologies.</rdfs:comment>
        <rdfs:label>PSS-Use Condition</rdfs:label>
    </owl:Class>
    


    <!-- https://gitlab.atb-bremen.de/atb/pss-ontology/PSS-ontology-2#PSSBusinessProcess -->

    <owl:Class rdf:about="https://gitlab.atb-bremen.de/atb/pss-ontology/PSS-ontology-2#PSSBusinessProcess">
        <rdfs:subClassOf rdf:resource="http://purl.obolibrary.org/obo/BFO_0000015"/>
        <obo:IAO_0000115>PSS Business Process is a process in which PSS is developed, implemented, distributed and used.</obo:IAO_0000115>
        <obo:IAO_0000118>A PSS business process is a planned process that realizes a function which is related to generation of a system which bears a PSS role</obo:IAO_0000118>
        <dc:contributor>ATB - EPFL</dc:contributor>
        <rdfs:label>PSS business process</rdfs:label>
    </owl:Class>
    


    <!-- https://gitlab.atb-bremen.de/atb/pss-ontology/PSS-ontology-2#PSSNon-ConsumableResourceRole -->

    <owl:Class rdf:about="https://gitlab.atb-bremen.de/atb/pss-ontology/PSS-ontology-2#PSSNon-ConsumableResourceRole">
        <rdfs:subClassOf rdf:resource="http://purl.obolibrary.org/obo/BFO_0000023"/>
        <obo:IAO_0000112>infrastructure, machines</obo:IAO_0000112>
        <CommonCoreOntologies:definition>A BFO:role that is borne by a BFO:material, when that entity is intended to be used but quantity is not reduced in a PSS process</CommonCoreOntologies:definition>
        <rdfs:label>PSS Non-Consumable Resource Role</rdfs:label>
    </owl:Class>
    


    <!-- https://gitlab.atb-bremen.de/atb/pss-ontology/PSS-ontology-2#PSS_Condition -->

    <owl:Class rdf:about="https://gitlab.atb-bremen.de/atb/pss-ontology/PSS-ontology-2#PSS_Condition">
        <rdfs:subClassOf rdf:resource="http://purl.obolibrary.org/obo/BFO_0000141"/>
        <obo:IAO_0000115>PSS Condition is a non-material entity that describes the situation around PSS.</obo:IAO_0000115>
        <dc:contributor>ATB - EPFL</dc:contributor>
        <rdfs:label>PSS Condition</rdfs:label>
    </owl:Class>
    


    <!-- https://gitlab.atb-bremen.de/atb/pss-ontology/PSS-ontology-2#PSS_Feature -->

    <owl:Class rdf:about="https://gitlab.atb-bremen.de/atb/pss-ontology/PSS-ontology-2#PSS_Feature">
        <rdfs:subClassOf rdf:resource="https://gitlab.atb-bremen.de/atb/pss-ontology/PSS-ontology-2#Feature"/>
        <obo:IAO_0000115>PSS Feature is a Feature that describes an aspect or attribute related to the PSS.</obo:IAO_0000115>
        <dc:contributor>ATB - EPFL</dc:contributor>
        <rdfs:label>PSS Feature</rdfs:label>
    </owl:Class>
    


    <!-- https://gitlab.atb-bremen.de/atb/pss-ontology/PSS-ontology-2#PSS_Lifecycle -->

    <owl:Class rdf:about="https://gitlab.atb-bremen.de/atb/pss-ontology/PSS-ontology-2#PSS_Lifecycle">
        <rdfs:subClassOf rdf:resource="https://gitlab.atb-bremen.de/atb/pss-ontology/PSS-ontology-2#Lifecycle"/>
        <obo:IAO_0000115>PSS Lifecycle is a Lifecycle that includes the PSS processes from the idea conceptualisation to its end-of-life, referring to the PSS Lifecycle Model in conjunction with time.</obo:IAO_0000115>
        <dc:contributor>ATB - EPFL</dc:contributor>
        <rdfs:label>PSS Lifecycle</rdfs:label>
    </owl:Class>
    


    <!-- https://gitlab.atb-bremen.de/atb/pss-ontology/PSS-ontology-2#PSS_Lifecycle_Model -->

    <owl:Class rdf:about="https://gitlab.atb-bremen.de/atb/pss-ontology/PSS-ontology-2#PSS_Lifecycle_Model">
        <rdfs:subClassOf rdf:resource="https://gitlab.atb-bremen.de/atb/pss-ontology/PSS-ontology-2#Lifecycle_Model"/>
        <obo:IAO_0000115>PSS Lifecycle Model is the Lifecycle Model that refers to the different stages of the life of PSS.</obo:IAO_0000115>
        <dc:contributor>ATB - EPFL</dc:contributor>
        <rdfs:label>PSS Lifecycle Model</rdfs:label>
    </owl:Class>
    


    <!-- https://gitlab.atb-bremen.de/atb/pss-ontology/PSS-ontology-2#PSS_Provider -->

    <owl:Class rdf:about="https://gitlab.atb-bremen.de/atb/pss-ontology/PSS-ontology-2#PSS_Provider">
        <rdfs:subClassOf rdf:resource="https://gitlab.atb-bremen.de/atb/pss-ontology/PSS-ontology-2#Supplier/Provider/Vendor"/>
        <obo:IAO_0000115>PSS Provider is a Supplier/ Provider/Vendor that offers PSS and owns intellectual property rights (IPR) on PSS offer.</obo:IAO_0000115>
        <dc:contributor>ATB - EPFL</dc:contributor>
        <rdfs:label>PSS Provider</rdfs:label>
    </owl:Class>
    


    <!-- https://gitlab.atb-bremen.de/atb/pss-ontology/PSS-ontology-2#PSS_Role -->

    <owl:Class rdf:about="https://gitlab.atb-bremen.de/atb/pss-ontology/PSS-ontology-2#PSS_Role">
        <rdfs:subClassOf rdf:resource="http://purl.obolibrary.org/obo/BFO_0000023"/>
        <obo:IAO_0000115>PSS role is a role that borne by set of at least an entity that is the specified output of a product production process and at least an entity that is the specified output of a service development process, and may include material entity that is used in PSS processes and actors that are involved in PSS processes. This set is intended to satisfy a need of the market, to be competitive, and jointly fulfil customer’s needs.</obo:IAO_0000115>
        <obo:IAO_0000118>PSS role is a role that borne by set of at least an entity that is the specified output of a product production process and at least an entity that is the specified output of a service development process.</obo:IAO_0000118>
        <dc:contributor>ATB - EPFL</dc:contributor>
        <rdfs:comment>PSS Role is an optional characteristic of a system combining products and services, aiming to satisfy a need of the market (e.g. to be sold in order to provide profit and support customers by covering their needs).</rdfs:comment>
        <rdfs:label>PSS Role</rdfs:label>
    </owl:Class>
    


    <!-- https://gitlab.atb-bremen.de/atb/pss-ontology/PSS-ontology-2#PSS_Type -->

    <owl:Class rdf:about="https://gitlab.atb-bremen.de/atb/pss-ontology/PSS-ontology-2#PSS_Type">
        <rdfs:subClassOf rdf:resource="https://gitlab.atb-bremen.de/atb/pss-ontology/PSS-ontology-2#PSS_Feature"/>
        <obo:IAO_0000112>Typical examples of PSS with a different type feature are e.g. the product- oriented PSS, the result-oriented PSS and the use-oriented PSS.</obo:IAO_0000112>
        <obo:IAO_0000115>PSS-Type Feature is a PSS Feature that refers to characteristics that define the subgroup where a PSS belongs to, and describe the specific focus (orientation or aim) of a PSS, such as to engage the customer with services, or to increase the sales of a product.</obo:IAO_0000115>
        <dc:contributor>ATB - EPFL</dc:contributor>
        <rdfs:label>PSS Type Feature</rdfs:label>
    </owl:Class>
    


    <!-- https://gitlab.atb-bremen.de/atb/pss-ontology/PSS-ontology-2#Process_Definition -->

    <owl:Class rdf:about="https://gitlab.atb-bremen.de/atb/pss-ontology/PSS-ontology-2#Process_Definition">
        <rdfs:subClassOf rdf:resource="http://purl.obolibrary.org/obo/BFO_0000017"/>
        <obo:IAO_0000115>Process Definition is a structured set of activities designed to accomplish a specific objective [4]. For example, the Process Definition can be the manufacturing process where the equipment is manufactured, or the process where the equipment is used, or the development process where products, services or PSS are being developed etc.</obo:IAO_0000115>
        <obo:IAO_0000119>Resources:

4. Wikipedia contributors, &apos;Business process&apos;, Wikipedia, The Free Encyclopaedia, 17 July 2017, 11:25 UTC, &lt;https://en.wikipedia.org/w/index.php?title=Business_process&amp;oldid=790986805&gt; [accessed 20 July 2017]</obo:IAO_0000119>
        <dc:contributor>ATB - EPFL</dc:contributor>
        <rdfs:comment>NOTE: Relation to BFO - Under continuant the process (definition) is being modelled as part of the PSS environment without including the time duration in which this process is valid. The time aspect of the process is included, however, as part of the modelling as occurrent.</rdfs:comment>
        <rdfs:label>Process Definition</rdfs:label>
    </owl:Class>
    


    <!-- https://gitlab.atb-bremen.de/atb/pss-ontology/PSS-ontology-2#Product -->

    <owl:Class rdf:about="https://gitlab.atb-bremen.de/atb/pss-ontology/PSS-ontology-2#Product">
        <rdfs:subClassOf rdf:resource="https://gitlab.atb-bremen.de/atb/pss-ontology/PSS-ontology-2#Material_Object"/>
        <obo:IAO_0000115>Product (for manufacturing industry) is a Material Object, manufactured to satisfy a need of the market [5] (e.g. to be sold in order to provide profit and support customers by covering their needs).</obo:IAO_0000115>
        <obo:IAO_0000118>A PSS:product is a commercially distributed good that is a tangible property and (1) the output of a fabrication, manufacturing, or production process, and (2) something that passes through a distribution channel before being consumed or used&apos;</obo:IAO_0000118>
        <obo:IAO_0000118>A Product is an entity that bears a product role</obo:IAO_0000118>
        <obo:IAO_0000119>5. Wikipedia contributors, &apos;Product&apos;, Wikipedia, The Free Encyclopaedia, 10 July 2017, 15:21 UTC, &lt;https://en.wikipedia.org/w/index.php?title=Product&amp;oldid=789934020&gt; [accessed 20 July 2017]</obo:IAO_0000119>
        <dc:contributor>ATB - EPFL</dc:contributor>
        <rdfs:comment>It may serve as an interface class for merging with other ontologies.</rdfs:comment>
        <rdfs:label>Product</rdfs:label>
    </owl:Class>
    


    <!-- https://gitlab.atb-bremen.de/atb/pss-ontology/PSS-ontology-2#ProductProductionProcess -->

    <owl:Class rdf:about="https://gitlab.atb-bremen.de/atb/pss-ontology/PSS-ontology-2#ProductProductionProcess">
        <rdfs:subClassOf rdf:resource="http://purl.obolibrary.org/obo/BFO_0000015"/>
        <dc:contributor>A product production process is a planned process that has output some continuant, where the continuant did not exist prior to the planned process, and where the agent who performs the process intends for the continuant to bear a product role.</dc:contributor>
        <dc:contributor>ATB - EPFL</dc:contributor>
        <rdfs:label>Product Production Process</rdfs:label>
    </owl:Class>
    


    <!-- https://gitlab.atb-bremen.de/atb/pss-ontology/PSS-ontology-2#Product_Component -->

    <owl:Class rdf:about="https://gitlab.atb-bremen.de/atb/pss-ontology/PSS-ontology-2#Product_Component">
        <rdfs:subClassOf rdf:resource="https://gitlab.atb-bremen.de/atb/pss-ontology/PSS-ontology-2#Material_Object"/>
        <obo:IAO_0000115>Product Component is a Material Object which is part of the Product. It can be itself a manufactured product, but for the offered product within the scope of PSS, its existence only has a meaning as part of the product.</obo:IAO_0000115>
        <dc:contributor>ATB - EPFL</dc:contributor>
        <rdfs:comment>It may serve as an interface class for merging with other ontologies.</rdfs:comment>
        <rdfs:label>Product Component</rdfs:label>
    </owl:Class>
    


    <!-- https://gitlab.atb-bremen.de/atb/pss-ontology/PSS-ontology-2#Product_Data -->

    <owl:Class rdf:about="https://gitlab.atb-bremen.de/atb/pss-ontology/PSS-ontology-2#Product_Data">
        <rdfs:subClassOf rdf:resource="https://gitlab.atb-bremen.de/atb/pss-ontology/PSS-ontology-2#Data"/>
        <obo:IAO_0000115>Product Data are PSS Source-Data used in the scope of PSS, and refer specifically to the product part of PSS.</obo:IAO_0000115>
        <dc:contributor>ATB - EPFL</dc:contributor>
        <rdfs:label>Product Data</rdfs:label>
    </owl:Class>
    


    <!-- https://gitlab.atb-bremen.de/atb/pss-ontology/PSS-ontology-2#Product_Extension_Service -->

    <owl:Class rdf:about="https://gitlab.atb-bremen.de/atb/pss-ontology/PSS-ontology-2#Product_Extension_Service">
        <rdfs:subClassOf rdf:resource="https://gitlab.atb-bremen.de/atb/pss-ontology/PSS-ontology-2#Service"/>
        <obo:IAO_0000115>Product Extension Service is a Service which adds additional value to the product.</obo:IAO_0000115>
        <dc:contributor>ATB - EPFL</dc:contributor>
        <rdfs:label>Product Extension Service</rdfs:label>
    </owl:Class>
    


    <!-- https://gitlab.atb-bremen.de/atb/pss-ontology/PSS-ontology-2#Product_Extension_Service_Offer -->

    <owl:Class rdf:about="https://gitlab.atb-bremen.de/atb/pss-ontology/PSS-ontology-2#Product_Extension_Service_Offer">
        <rdfs:subClassOf rdf:resource="https://gitlab.atb-bremen.de/atb/pss-ontology/PSS-ontology-2#Service_Offer"/>
        <obo:IAO_0000115>Product-Extension Service-Offer is a Service Offer which adds value to the product.</obo:IAO_0000115>
        <dc:contributor>ATB - EPFL</dc:contributor>
        <rdfs:label>Product Extension Service Offer</rdfs:label>
    </owl:Class>
    


    <!-- https://gitlab.atb-bremen.de/atb/pss-ontology/PSS-ontology-2#Product_Feature -->

    <owl:Class rdf:about="https://gitlab.atb-bremen.de/atb/pss-ontology/PSS-ontology-2#Product_Feature">
        <rdfs:subClassOf rdf:resource="https://gitlab.atb-bremen.de/atb/pss-ontology/PSS-ontology-2#Feature"/>
        <obo:IAO_0000115>Product Feature is a Feature that describes an aspect, or attribute, related to the product within the PSS scope.</obo:IAO_0000115>
        <dc:contributor>ATB - EPFL</dc:contributor>
        <rdfs:label>Product Feature</rdfs:label>
    </owl:Class>
    


    <!-- https://gitlab.atb-bremen.de/atb/pss-ontology/PSS-ontology-2#Product_Integrated_Set -->

    <owl:Class rdf:about="https://gitlab.atb-bremen.de/atb/pss-ontology/PSS-ontology-2#Product_Integrated_Set">
        <rdfs:subClassOf rdf:resource="https://gitlab.atb-bremen.de/atb/pss-ontology/PSS-ontology-2#Material_Object"/>
        <obo:IAO_0000115>Product Integrated Set is a Material Object that consists of a set of products needed to jointly fulfil users’ needs.</obo:IAO_0000115>
        <dc:contributor>ATB - EPFL</dc:contributor>
        <rdfs:label>Product Integrated Set</rdfs:label>
    </owl:Class>
    


    <!-- https://gitlab.atb-bremen.de/atb/pss-ontology/PSS-ontology-2#Product_Lifecycle -->

    <owl:Class rdf:about="https://gitlab.atb-bremen.de/atb/pss-ontology/PSS-ontology-2#Product_Lifecycle">
        <rdfs:subClassOf rdf:resource="https://gitlab.atb-bremen.de/atb/pss-ontology/PSS-ontology-2#Lifecycle"/>
        <obo:IAO_0000115>Product Lifecycle is a Lifecycle that includes only the Product-specific processes, in the scope of PSS. It refers to the Product Lifecycle Model in conjunction with time.</obo:IAO_0000115>
        <dc:contributor>ATB - EPFL</dc:contributor>
        <rdfs:label>Product Lifecycle</rdfs:label>
    </owl:Class>
    


    <!-- https://gitlab.atb-bremen.de/atb/pss-ontology/PSS-ontology-2#Product_Lifecycle_Model -->

    <owl:Class rdf:about="https://gitlab.atb-bremen.de/atb/pss-ontology/PSS-ontology-2#Product_Lifecycle_Model">
        <rdfs:subClassOf rdf:resource="https://gitlab.atb-bremen.de/atb/pss-ontology/PSS-ontology-2#Lifecycle_Model"/>
        <obo:IAO_0000115>Product Lifecycle Model is a Lifecycle Model that refers to the product within the scope of PSS.</obo:IAO_0000115>
        <dc:contributor>ATB - EPFL</dc:contributor>
        <rdfs:label>Product Lifecycle Model</rdfs:label>
    </owl:Class>
    


    <!-- https://gitlab.atb-bremen.de/atb/pss-ontology/PSS-ontology-2#Product_Provider -->

    <owl:Class rdf:about="https://gitlab.atb-bremen.de/atb/pss-ontology/PSS-ontology-2#Product_Provider">
        <rdfs:subClassOf rdf:resource="https://gitlab.atb-bremen.de/atb/pss-ontology/PSS-ontology-2#Supplier/Provider/Vendor"/>
        <obo:IAO_0000115>Product Provider is a Supplier/ provider/vendor that both produces and sells a product, or only sells it.</obo:IAO_0000115>
        <dc:contributor>ATB - EPFL</dc:contributor>
        <rdfs:label>Product Provider</rdfs:label>
    </owl:Class>
    


    <!-- https://gitlab.atb-bremen.de/atb/pss-ontology/PSS-ontology-2#Product_Role -->

    <owl:Class rdf:about="https://gitlab.atb-bremen.de/atb/pss-ontology/PSS-ontology-2#Product_Role">
        <rdfs:subClassOf rdf:resource="http://purl.obolibrary.org/obo/BFO_0000023"/>
        <obo:IAO_0000115>A Product Role is a role borne by an entity that is the specified output of a product production process</obo:IAO_0000115>
        <obo:IAO_0000118>A Product Role is a role borne by an entity that is the specified output of a product production process Role that is borne by a BFO: Continuant intended to be sold (and bearing some economic value, the value can be zero, positive, or negative)</obo:IAO_0000118>
        <obo:IAO_0000118>Product Role is an optional characteristic of a material object manufactured to satisfy a need of the market (e.g. to be sold in order to provide profit and support customers by covering their needs).</obo:IAO_0000118>
        <dc:contributor>ATB - EPFL</dc:contributor>
        <rdfs:label>Product Role</rdfs:label>
    </owl:Class>
    


    <!-- https://gitlab.atb-bremen.de/atb/pss-ontology/PSS-ontology-2#Product_Type_Feature -->

    <owl:Class rdf:about="https://gitlab.atb-bremen.de/atb/pss-ontology/PSS-ontology-2#Product_Type_Feature">
        <rdfs:subClassOf rdf:resource="https://gitlab.atb-bremen.de/atb/pss-ontology/PSS-ontology-2#Product_Feature"/>
        <obo:IAO_0000115>Product-Type Feature is a Product Feature that refers to characteristics that define the subgroup where a product belongs to.</obo:IAO_0000115>
        <dc:contributor>ATB - EPFL</dc:contributor>
        <rdfs:comment>Product type is sector or company specific. These are features which characterise the specific type (subgroup) of the product.</rdfs:comment>
        <rdfs:label>Product Type Feature</rdfs:label>
    </owl:Class>
    


    <!-- https://gitlab.atb-bremen.de/atb/pss-ontology/PSS-ontology-2#PssConsumableResource -->

    <owl:Class rdf:about="https://gitlab.atb-bremen.de/atb/pss-ontology/PSS-ontology-2#PssConsumableResource">
        <rdfs:subClassOf rdf:resource="https://gitlab.atb-bremen.de/atb/pss-ontology/PSS-ontology-2#Resource"/>
        <CommonCoreOntologies:definition>Is a IOF:Resource that can bear a PSS Consumable Resource Role</CommonCoreOntologies:definition>
        <rdfs:label>PSS Consumable Resource</rdfs:label>
    </owl:Class>
    


    <!-- https://gitlab.atb-bremen.de/atb/pss-ontology/PSS-ontology-2#PssConsumableResourceRole -->

    <owl:Class rdf:about="https://gitlab.atb-bremen.de/atb/pss-ontology/PSS-ontology-2#PssConsumableResourceRole">
        <rdfs:subClassOf rdf:resource="http://purl.obolibrary.org/obo/BFO_0000023"/>
        <CommonCoreOntologies:definition>A BFO:role that is borne by a BFO:material, when that entity is intended to be consumed/transformed in a PSS process. The quantities of resources is reduced after use (in a PSS process).</CommonCoreOntologies:definition>
        <rdfs:label>PSS Consumable Resource Role</rdfs:label>
    </owl:Class>
    


    <!-- https://gitlab.atb-bremen.de/atb/pss-ontology/PSS-ontology-2#PssNon-ConsumableResource -->

    <owl:Class rdf:about="https://gitlab.atb-bremen.de/atb/pss-ontology/PSS-ontology-2#PssNon-ConsumableResource">
        <rdfs:subClassOf rdf:resource="https://gitlab.atb-bremen.de/atb/pss-ontology/PSS-ontology-2#Resource"/>
        <obo:IAO_0000118>PSS Non-Consumable Resource</obo:IAO_0000118>
        <CommonCoreOntologies:definition>PSS Infrastructure is a Resource including the physical (e.g. buildings or machines, computers), and organisational (e.g. communication networks) means used to assist in development and delivering of the Product and Services.</CommonCoreOntologies:definition>
        <rdfs:label>PSS Infrastructure</rdfs:label>
    </owl:Class>
    


    <!-- https://gitlab.atb-bremen.de/atb/pss-ontology/PSS-ontology-2#Requirement -->

    <owl:Class rdf:about="https://gitlab.atb-bremen.de/atb/pss-ontology/PSS-ontology-2#Requirement">
        <rdfs:subClassOf rdf:resource="https://gitlab.atb-bremen.de/atb/pss-ontology/PSS-ontology-2#Information"/>
        <obo:IAO_0000115>Requirement is PSS Information that depicts the aspects which are necessary for the design, development or offer of PSS. Requirement is defined by the Stakeholder.</obo:IAO_0000115>
        <dc:contributor>ATB - EPFL</dc:contributor>
        <rdfs:comment>Requirement can be further extended according to the ISO standard or other System Engineering references.
Here it serves as an interface class for merging with other ontologies.</rdfs:comment>
    </owl:Class>
    


    <!-- https://gitlab.atb-bremen.de/atb/pss-ontology/PSS-ontology-2#Resource -->

    <owl:Class rdf:about="https://gitlab.atb-bremen.de/atb/pss-ontology/PSS-ontology-2#Resource">
        <rdfs:subClassOf rdf:resource="http://purl.obolibrary.org/obo/BFO_0000031"/>
        <obo:IAO_0000115>Resource is a mean (source) that can be used for the design, development, offer and delivery of a PSS, from which benefit can be produced [2].</obo:IAO_0000115>
        <obo:IAO_0000119>Resources:

2.  Wikipedia contributors, &apos;Resource&apos;, Wikipedia, The Free Encyclopaedia, 27 June 2017, 08:20 UTC, &lt;https://en.wikipedia.org/w/index.php?title=Resource&amp;oldid=787741678&gt; [accessed 20 July 2017]</obo:IAO_0000119>
        <dc:contributor>ATB - EPFL</dc:contributor>
        <rdfs:label>Resource</rdfs:label>
    </owl:Class>
    


    <!-- https://gitlab.atb-bremen.de/atb/pss-ontology/PSS-ontology-2#Service -->

    <owl:Class rdf:about="https://gitlab.atb-bremen.de/atb/pss-ontology/PSS-ontology-2#Service">
        <rdfs:subClassOf rdf:resource="http://purl.obolibrary.org/obo/BFO_0000015"/>
        <obo:IAO_0000115>Service is a planned Process which has agents Service Provider and agent Consumer and the Process fulfills a need of the Consumer and where the act of providing coincide with the act of consumption.</obo:IAO_0000115>
        <obo:IAO_0000116>Old definition: Service is a Process made for, and driven by customers, with economic value, and refers to the Service Offer entity in conjunction with time.</obo:IAO_0000116>
        <dc:contributor>ATB - EPFL</dc:contributor>
        <rdfs:comment>This is an interface class to other ontologies.</rdfs:comment>
    </owl:Class>
    


    <!-- https://gitlab.atb-bremen.de/atb/pss-ontology/PSS-ontology-2#ServiceResource -->

    <owl:Class rdf:about="https://gitlab.atb-bremen.de/atb/pss-ontology/PSS-ontology-2#ServiceResource">
        <rdfs:subClassOf rdf:resource="http://purl.obolibrary.org/obo/BFO_0000031"/>
        <obo:IAO_0000115>Service resource =def. continuant that bears a service resource role.</obo:IAO_0000115>
        <rdfs:label>Service Resource</rdfs:label>
    </owl:Class>
    


    <!-- https://gitlab.atb-bremen.de/atb/pss-ontology/PSS-ontology-2#ServiceResourceRole -->

    <owl:Class rdf:about="https://gitlab.atb-bremen.de/atb/pss-ontology/PSS-ontology-2#ServiceResourceRole">
        <rdfs:subClassOf rdf:resource="http://purl.obolibrary.org/obo/BFO_0000023"/>
        <obo:IAO_0000115>Role that inheres in an independent continuant where that continuant bears a disposition that, if realized, is realized in a service development and deployment/use processes</obo:IAO_0000115>
        <dc:contributor>ATB - EPFL</dc:contributor>
        <rdfs:label>Service Resource Role</rdfs:label>
    </owl:Class>
    


    <!-- https://gitlab.atb-bremen.de/atb/pss-ontology/PSS-ontology-2#Service_Component -->

    <owl:Class rdf:about="https://gitlab.atb-bremen.de/atb/pss-ontology/PSS-ontology-2#Service_Component">
        <rdfs:subClassOf rdf:resource="http://purl.obolibrary.org/obo/BFO_0000015"/>
        <obo:IAO_0000115>Service Component is a Process, part of a Service, and refers to the Service Offer Component in conjunction with time.</obo:IAO_0000115>
        <dc:contributor>ATB - EPFL</dc:contributor>
        <rdfs:label>Service Component</rdfs:label>
    </owl:Class>
    


    <!-- https://gitlab.atb-bremen.de/atb/pss-ontology/PSS-ontology-2#Service_Data -->

    <owl:Class rdf:about="https://gitlab.atb-bremen.de/atb/pss-ontology/PSS-ontology-2#Service_Data">
        <rdfs:subClassOf rdf:resource="https://gitlab.atb-bremen.de/atb/pss-ontology/PSS-ontology-2#Data"/>
        <obo:IAO_0000115>Service Data are PSS Source Data used in the scope of PSS, and are generated specifically in the service part of PSS (e.g. data generated during a call in the service centre).</obo:IAO_0000115>
        <dc:contributor>ATB - EPFL</dc:contributor>
        <rdfs:label>Service Data</rdfs:label>
    </owl:Class>
    


    <!-- https://gitlab.atb-bremen.de/atb/pss-ontology/PSS-ontology-2#Service_Feature -->

    <owl:Class rdf:about="https://gitlab.atb-bremen.de/atb/pss-ontology/PSS-ontology-2#Service_Feature">
        <rdfs:subClassOf rdf:resource="https://gitlab.atb-bremen.de/atb/pss-ontology/PSS-ontology-2#Feature"/>
        <obo:IAO_0000115>Service-Offer Feature is a Feature that describes an aspect or attribute related to the service within the PSS scope.</obo:IAO_0000115>
        <dc:contributor>ATB - EPFL</dc:contributor>
        <rdfs:label>Service Offer Feature</rdfs:label>
    </owl:Class>
    


    <!-- https://gitlab.atb-bremen.de/atb/pss-ontology/PSS-ontology-2#Service_Lifecycle -->

    <owl:Class rdf:about="https://gitlab.atb-bremen.de/atb/pss-ontology/PSS-ontology-2#Service_Lifecycle">
        <rdfs:subClassOf rdf:resource="https://gitlab.atb-bremen.de/atb/pss-ontology/PSS-ontology-2#Lifecycle"/>
        <obo:IAO_0000115>Service Lifecycle is a Lifecycle that includes only the service-specific processes, in the scope of PSS. It refers to the Service Lifecycle Model in conjunction with time.</obo:IAO_0000115>
        <dc:contributor>ATB - EPFL</dc:contributor>
        <rdfs:label>Service Lifecycle</rdfs:label>
    </owl:Class>
    


    <!-- https://gitlab.atb-bremen.de/atb/pss-ontology/PSS-ontology-2#Service_Lifecycle_Model -->

    <owl:Class rdf:about="https://gitlab.atb-bremen.de/atb/pss-ontology/PSS-ontology-2#Service_Lifecycle_Model">
        <rdfs:subClassOf rdf:resource="https://gitlab.atb-bremen.de/atb/pss-ontology/PSS-ontology-2#Lifecycle_Model"/>
        <obo:IAO_0000115>Service Lifecycle Model is the Lifecycle Model that refers to the Service Offer within the scope of PSS.</obo:IAO_0000115>
        <dc:contributor>ATB - EPFL</dc:contributor>
        <rdfs:label>Service Lifecycle Model</rdfs:label>
    </owl:Class>
    


    <!-- https://gitlab.atb-bremen.de/atb/pss-ontology/PSS-ontology-2#Service_Offer -->

    <owl:Class rdf:about="https://gitlab.atb-bremen.de/atb/pss-ontology/PSS-ontology-2#Service_Offer">
        <rdfs:subClassOf rdf:resource="https://gitlab.atb-bremen.de/atb/pss-ontology/PSS-ontology-2#Process_Definition"/>
        <obo:IAO_0000115>Service Offer is a Process Definition referring to a set of non-tangible entities (activities, software modules etc.), related to the service part of PSS, which aims to satisfy a need of the market (e.g. to be sold in order to provide profit and support customers by covering their needs).</obo:IAO_0000115>
        <obo:IAO_0000118>Service Offer is a description/definition of a Service (all the activities that have to be done to fulfil the Service)</obo:IAO_0000118>
        <dc:contributor>ATB - EPFL</dc:contributor>
        <rdfs:comment>This is an interface class to other ontologies.</rdfs:comment>
        <rdfs:label>Service Offer</rdfs:label>
    </owl:Class>
    


    <!-- https://gitlab.atb-bremen.de/atb/pss-ontology/PSS-ontology-2#Service_Offer_Component -->

    <owl:Class rdf:about="https://gitlab.atb-bremen.de/atb/pss-ontology/PSS-ontology-2#Service_Offer_Component">
        <rdfs:subClassOf rdf:resource="https://gitlab.atb-bremen.de/atb/pss-ontology/PSS-ontology-2#Process_Definition"/>
        <obo:IAO_0000115>Service-Offer Component is a Process Definition which is part of a Service Offer. It can be itself a service, but for the offered service within the scope of PSS, its existence only has a meaning as part of the PSS service offer.</obo:IAO_0000115>
        <dc:contributor>ATB - EPFL</dc:contributor>
        <rdfs:label>Service Offer Component</rdfs:label>
    </owl:Class>
    


    <!-- https://gitlab.atb-bremen.de/atb/pss-ontology/PSS-ontology-2#Service_Offer_Integrated_set -->

    <owl:Class rdf:about="https://gitlab.atb-bremen.de/atb/pss-ontology/PSS-ontology-2#Service_Offer_Integrated_set">
        <rdfs:subClassOf rdf:resource="https://gitlab.atb-bremen.de/atb/pss-ontology/PSS-ontology-2#Process_Definition"/>
        <obo:IAO_0000115>Service Offer Integrated-Set is a Process Definition that refers to a set of Service Offers, needed to jointly fulfil users’ needs.</obo:IAO_0000115>
        <dc:contributor>ATB - EPFL</dc:contributor>
        <rdfs:label>Service Offer Integrated Set</rdfs:label>
    </owl:Class>
    


    <!-- https://gitlab.atb-bremen.de/atb/pss-ontology/PSS-ontology-2#Service_Offer_Role -->

    <owl:Class rdf:about="https://gitlab.atb-bremen.de/atb/pss-ontology/PSS-ontology-2#Service_Offer_Role">
        <rdfs:subClassOf rdf:resource="http://purl.obolibrary.org/obo/BFO_0000023"/>
        <obo:IAO_0000115>Service Offer Role is an optional characteristic of a non-tangible entity that aims to satisfy a need of the market (e.g. to be sold in order to provide profit and support customers by covering their needs).</obo:IAO_0000115>
        <obo:IAO_0000118>A service offer role is a role borne by an entity that is the specified output of a service offer development process</obo:IAO_0000118>
        <dc:contributor>ATB - EPFL</dc:contributor>
        <rdfs:label>Service Offer Role</rdfs:label>
    </owl:Class>
    


    <!-- https://gitlab.atb-bremen.de/atb/pss-ontology/PSS-ontology-2#Service_Provider -->

    <owl:Class rdf:about="https://gitlab.atb-bremen.de/atb/pss-ontology/PSS-ontology-2#Service_Provider">
        <rdfs:subClassOf rdf:resource="https://gitlab.atb-bremen.de/atb/pss-ontology/PSS-ontology-2#Supplier/Provider/Vendor"/>
        <obo:IAO_0000115>Service Provider is a Supplier/ provider/vendor that offers a service.</obo:IAO_0000115>
        <dc:contributor>ATB - EPFL</dc:contributor>
        <rdfs:label>Service Provider</rdfs:label>
    </owl:Class>
    


    <!-- https://gitlab.atb-bremen.de/atb/pss-ontology/PSS-ontology-2#Service_Type_Feature -->

    <owl:Class rdf:about="https://gitlab.atb-bremen.de/atb/pss-ontology/PSS-ontology-2#Service_Type_Feature">
        <rdfs:subClassOf rdf:resource="https://gitlab.atb-bremen.de/atb/pss-ontology/PSS-ontology-2#Service_Feature"/>
        <obo:IAO_0000115>Service-Type Feature is a Service Feature that refers to characteristics that define the subgroup where a service belongs to.</obo:IAO_0000115>
        <dc:contributor>ATB - EPFL</dc:contributor>
        <rdfs:comment>Service type is sectorial or company specific</rdfs:comment>
        <rdfs:label>Service Type Feature</rdfs:label>
    </owl:Class>
    


    <!-- https://gitlab.atb-bremen.de/atb/pss-ontology/PSS-ontology-2#Software_Infrastructure -->

    <owl:Class rdf:about="https://gitlab.atb-bremen.de/atb/pss-ontology/PSS-ontology-2#Software_Infrastructure">
        <rdfs:subClassOf rdf:resource="https://gitlab.atb-bremen.de/atb/pss-ontology/PSS-ontology-2#Infrastructure"/>
        <obo:IAO_0000115>Software is an infrastructure that refers to the non-material aspects (resources) necessary for the design, development, delivery and operation of the PSS.</obo:IAO_0000115>
        <dc:contributor>ATB - EPFL</dc:contributor>
        <rdfs:label>software infrastucture</rdfs:label>
    </owl:Class>
    


    <!-- https://gitlab.atb-bremen.de/atb/pss-ontology/PSS-ontology-2#Software_Log -->

    <owl:Class rdf:about="https://gitlab.atb-bremen.de/atb/pss-ontology/PSS-ontology-2#Software_Log">
        <rdfs:subClassOf rdf:resource="https://gitlab.atb-bremen.de/atb/pss-ontology/PSS-ontology-2#Product_Data"/>
        <obo:IAO_0000115>Digital Log Data are Product Data generated from a software element, part of the product.</obo:IAO_0000115>
        <dc:contributor>ATB - EPFL</dc:contributor>
        <rdfs:label>Digital Log Data</rdfs:label>
    </owl:Class>
    


    <!-- https://gitlab.atb-bremen.de/atb/pss-ontology/PSS-ontology-2#System -->

    <owl:Class rdf:about="https://gitlab.atb-bremen.de/atb/pss-ontology/PSS-ontology-2#System">
        <rdfs:subClassOf rdf:resource="http://purl.obolibrary.org/obo/BFO_0000020"/>
        <obo:IAO_0000115>System is a regularly interacting or interdependent group of items forming a unified whole [14]. Every system is delineated by its spatial and temporal boundaries, surrounded and influenced by its environment, described by its structure and purpose and expressed in its functioning [13]. In engineering and physics, a physical system is the portion of the universe that is being studied (of which a thermodynamic system is one major example). Engineering also has the concept of a system that refers to all of the parts and interactions between parts of a complex project. Systems engineering refers to the branch of engineering that studies how this type of system should be planned, designed, implemented, built, and maintained. System is a set of interacting elements [6] that, as a unity, affects the design/development of solutions. It is considered from the approach of System Engineering.</obo:IAO_0000115>
        <obo:IAO_0000119>Resources:

6. IEC, ISO. &quot;15288-2008. System engineering and software engineering–System life cycle processes.&quot; (2008), 
&lt; https://www.iso.org/standard/43564.html&gt; [accessed 20 July 2017]

13. Wikipedia contributors, &apos;System&apos;, Wikipedia, The Free Encyclopedia, 6 September 2017, 11:52 UTC, &lt;https://en.wikipedia.org/w/index.php?title=System&amp;oldid=799223483&gt; [accessed 20 September 2017]

14.  &quot;Definition of system&quot;. Merriam-Webster. Springfield, MA, USA. Retrieved 2016-10-09.</obo:IAO_0000119>
        <rdfs:comment>This is an interface class to other ontologies.</rdfs:comment>
        <rdfs:label>System</rdfs:label>
    </owl:Class>
    


    <!-- https://gitlab.atb-bremen.de/atb/pss-ontology/PSS-ontology-2#Stakeholder/Actor -->

    <owl:Class rdf:about="https://gitlab.atb-bremen.de/atb/pss-ontology/PSS-ontology-2#Stakeholder/Actor">
        <rdfs:subClassOf rdf:resource="http://purl.obolibrary.org/obo/BFO_0000040"/>
        <obo:IAO_0000115>Stakeholder/Actor is an entity that describes the humans (or beings) involved in a PSS (development, deployment, use etc.).</obo:IAO_0000115>
        <dc:contributor>ATB - EPFL</dc:contributor>
        <rdfs:comment>It may serve as an interface class for merging with other ontologies</rdfs:comment>
        <rdfs:label>Stakeholder/Actor</rdfs:label>
    </owl:Class>
    


    <!-- https://gitlab.atb-bremen.de/atb/pss-ontology/PSS-ontology-2#Supplier/Provider/Vendor -->

    <owl:Class rdf:about="https://gitlab.atb-bremen.de/atb/pss-ontology/PSS-ontology-2#Supplier/Provider/Vendor">
        <rdfs:subClassOf rdf:resource="https://gitlab.atb-bremen.de/atb/pss-ontology/PSS-ontology-2#Company"/>
        <obo:IAO_0000115>Supplier/Provider/Vendor is a Company that both produces and sells something (product, service, PSS), or only sells it.</obo:IAO_0000115>
        <dc:contributor>ATB - EPFL</dc:contributor>
        <rdfs:comment>Additional subclasses are possible, e.g. in DIVERSITY material supplier, component supplier etc.</rdfs:comment>
        <rdfs:label>Supplier/Provider/Vendor</rdfs:label>
    </owl:Class>
</rdf:RDF>



<!-- Generated by the OWL API (version 4.5.9.2019-02-01T07:24:44Z) https://github.com/owlcs/owlapi -->

