@prefix : <https://gitlab.atb-bremen.de/atb/pss-ontology/PSS-ontology-2#> .
@prefix dc: <http://purl.org/dc/elements/1.1/> .
@prefix obo: <http://purl.obolibrary.org/obo/> .
@prefix owl: <http://www.w3.org/2002/07/owl#> .
@prefix rdf: <http://www.w3.org/1999/02/22-rdf-syntax-ns#> .
@prefix xml: <http://www.w3.org/XML/1998/namespace> .
@prefix xsd: <http://www.w3.org/2001/XMLSchema#> .
@prefix foaf: <http://xmlns.com/foaf/0.1/> .
@prefix obda: <https://w3id.org/obda/vocabulary#> .
@prefix rdfs: <http://www.w3.org/2000/01/rdf-schema#> .
@prefix terms: <http://purl.org/dc/terms/> .
@prefix PSS-ontology-2: <http://www.semanticweb.org/atb/ontologies/2019/11/PSS-ontology-2#> .
@base <https://gitlab.atb-bremen.de/atb/pss-ontology/PSS-ontology-2> .

<https://gitlab.atb-bremen.de/atb/pss-ontology/PSS-ontology-2> rdf:type owl:Ontology ;
                                                                owl:versionIRI <https://gitlab.atb-bremen.de/atb/pss-ontology/PSS-ontology-2/0.2> ;
                                                                owl:imports <https://www.industrialontologies.org/core> .

#################################################################
#    Annotation properties
#################################################################

###  http://www.semanticweb.org/atb/ontologies/2019/11/PSS-ontology-2#description
PSS-ontology-2:description rdf:type owl:AnnotationProperty .


#################################################################
#    Object Properties
#################################################################

###  http://www.semanticweb.org/atb/ontologies/2019/11/PSS-ontology-2#BusinessCustomer_owns_PSS
PSS-ontology-2:BusinessCustomer_owns_PSS rdf:type owl:ObjectProperty .


###  http://www.semanticweb.org/atb/ontologies/2019/11/PSS-ontology-2#BusinessCustomer_owns_Product
PSS-ontology-2:BusinessCustomer_owns_Product rdf:type owl:ObjectProperty .


###  http://www.semanticweb.org/atb/ontologies/2019/11/PSS-ontology-2#BusinessCustomer_owns_ServiceOffer
PSS-ontology-2:BusinessCustomer_owns_ServiceOffer rdf:type owl:ObjectProperty .


###  http://www.semanticweb.org/atb/ontologies/2019/11/PSS-ontology-2#BusinessCustomer_provides_Feedback
PSS-ontology-2:BusinessCustomer_provides_Feedback rdf:type owl:ObjectProperty .


###  http://www.semanticweb.org/atb/ontologies/2019/11/PSS-ontology-2#Company_uses_Feedback
PSS-ontology-2:Company_uses_Feedback rdf:type owl:ObjectProperty .


###  http://www.semanticweb.org/atb/ontologies/2019/11/PSS-ontology-2#Company_uses_Guideline
PSS-ontology-2:Company_uses_Guideline rdf:type owl:ObjectProperty .


###  http://www.semanticweb.org/atb/ontologies/2019/11/PSS-ontology-2#Company_uses_Indicator
PSS-ontology-2:Company_uses_Indicator rdf:type owl:ObjectProperty .


###  http://www.semanticweb.org/atb/ontologies/2019/11/PSS-ontology-2#EmbeddedDataSourceComponent_generates_EmbeddedData
PSS-ontology-2:EmbeddedDataSourceComponent_generates_EmbeddedData rdf:type owl:ObjectProperty .


###  http://www.semanticweb.org/atb/ontologies/2019/11/PSS-ontology-2#Employee_uses_Infrastructure
PSS-ontology-2:Employee_uses_Infrastructure rdf:type owl:ObjectProperty .


###  http://www.semanticweb.org/atb/ontologies/2019/11/PSS-ontology-2#Feedback_refers_to_PSS
PSS-ontology-2:Feedback_refers_to_PSS rdf:type owl:ObjectProperty .


###  http://www.semanticweb.org/atb/ontologies/2019/11/PSS-ontology-2#Feedback_refers_to_Product
PSS-ontology-2:Feedback_refers_to_Product rdf:type owl:ObjectProperty .


###  http://www.semanticweb.org/atb/ontologies/2019/11/PSS-ontology-2#Feedback_refers_to_Service
PSS-ontology-2:Feedback_refers_to_Service rdf:type owl:ObjectProperty .


###  http://www.semanticweb.org/atb/ontologies/2019/11/PSS-ontology-2#IndividualCustomer_owns_PSS
PSS-ontology-2:IndividualCustomer_owns_PSS rdf:type owl:ObjectProperty .


###  http://www.semanticweb.org/atb/ontologies/2019/11/PSS-ontology-2#IndividualCustomer_owns_Product
PSS-ontology-2:IndividualCustomer_owns_Product rdf:type owl:ObjectProperty .


###  http://www.semanticweb.org/atb/ontologies/2019/11/PSS-ontology-2#IndividualCustomer_owns_ServiceOffer
PSS-ontology-2:IndividualCustomer_owns_ServiceOffer rdf:type owl:ObjectProperty .


###  http://www.semanticweb.org/atb/ontologies/2019/11/PSS-ontology-2#IndividualCustomer_provides_Feedback
PSS-ontology-2:IndividualCustomer_provides_Feedback rdf:type owl:ObjectProperty .


###  http://www.semanticweb.org/atb/ontologies/2019/11/PSS-ontology-2#IndividualPerson_provides_Feedback
PSS-ontology-2:IndividualPerson_provides_Feedback rdf:type owl:ObjectProperty .


###  http://www.semanticweb.org/atb/ontologies/2019/11/PSS-ontology-2#Lifecycle_implements_LifecycleModel
PSS-ontology-2:Lifecycle_implements_LifecycleModel rdf:type owl:ObjectProperty .


###  http://www.semanticweb.org/atb/ontologies/2019/11/PSS-ontology-2#PSSCondition_refers_to_PSS
PSS-ontology-2:PSSCondition_refers_to_PSS rdf:type owl:ObjectProperty .


###  http://www.semanticweb.org/atb/ontologies/2019/11/PSS-ontology-2#PSSProvider_supplies_PSS
PSS-ontology-2:PSSProvider_supplies_PSS rdf:type owl:ObjectProperty .


###  http://www.semanticweb.org/atb/ontologies/2019/11/PSS-ontology-2#PSS_belongsTo_PSSProvider
PSS-ontology-2:PSS_belongsTo_PSSProvider rdf:type owl:ObjectProperty ;
                                         rdfs:domain PSS-ontology-2:PSS ;
                                         rdfs:range PSS-ontology-2:PSS_Provider .


###  http://www.semanticweb.org/atb/ontologies/2019/11/PSS-ontology-2#PSS_exists_in_PSSLifecycle
PSS-ontology-2:PSS_exists_in_PSSLifecycle rdf:type owl:ObjectProperty .


###  http://www.semanticweb.org/atb/ontologies/2019/11/PSS-ontology-2#PSS_has_PSSFeature
PSS-ontology-2:PSS_has_PSSFeature rdf:type owl:ObjectProperty .


###  http://www.semanticweb.org/atb/ontologies/2019/11/PSS-ontology-2#PSS_has_PSSLifecycleModel
PSS-ontology-2:PSS_has_PSSLifecycleModel rdf:type owl:ObjectProperty .


###  http://www.semanticweb.org/atb/ontologies/2019/11/PSS-ontology-2#PSS_has_PSSRole
PSS-ontology-2:PSS_has_PSSRole rdf:type owl:ObjectProperty .


###  http://www.semanticweb.org/atb/ontologies/2019/11/PSS-ontology-2#PSS_implements_BusinessModel
PSS-ontology-2:PSS_implements_BusinessModel rdf:type owl:ObjectProperty .


###  http://www.semanticweb.org/atb/ontologies/2019/11/PSS-ontology-2#PSS_is_composed_of_Product
PSS-ontology-2:PSS_is_composed_of_Product rdf:type owl:ObjectProperty .


###  http://www.semanticweb.org/atb/ontologies/2019/11/PSS-ontology-2#PSS_is_composed_of_ServiceOffer
PSS-ontology-2:PSS_is_composed_of_ServiceOffer rdf:type owl:ObjectProperty .


###  http://www.semanticweb.org/atb/ontologies/2019/11/PSS-ontology-2#PSS_uses_Resource
PSS-ontology-2:PSS_uses_Resource rdf:type owl:ObjectProperty .


###  http://www.semanticweb.org/atb/ontologies/2019/11/PSS-ontology-2#Process_implements_ProcessDefinition
PSS-ontology-2:Process_implements_ProcessDefinition rdf:type owl:ObjectProperty .


###  http://www.semanticweb.org/atb/ontologies/2019/11/PSS-ontology-2#ProductExtensionServiceOffer_extends_Product
PSS-ontology-2:ProductExtensionServiceOffer_extends_Product rdf:type owl:ObjectProperty .


###  http://www.semanticweb.org/atb/ontologies/2019/11/PSS-ontology-2#ProductExtensionServiceOffer_uses_ProductData
PSS-ontology-2:ProductExtensionServiceOffer_uses_ProductData rdf:type owl:ObjectProperty .


###  http://www.semanticweb.org/atb/ontologies/2019/11/PSS-ontology-2#ProductIntegratedSet_is_composed_of_Products
PSS-ontology-2:ProductIntegratedSet_is_composed_of_Products rdf:type owl:ObjectProperty .


###  http://www.semanticweb.org/atb/ontologies/2019/11/PSS-ontology-2#ProductProvider_supplies_Product
PSS-ontology-2:ProductProvider_supplies_Product rdf:type owl:ObjectProperty .


###  http://www.semanticweb.org/atb/ontologies/2019/11/PSS-ontology-2#ProductProvider_supplies_ProductComponent
PSS-ontology-2:ProductProvider_supplies_ProductComponent rdf:type owl:ObjectProperty .


###  http://www.semanticweb.org/atb/ontologies/2019/11/PSS-ontology-2#Product_exists_in_ProductLifecycle
PSS-ontology-2:Product_exists_in_ProductLifecycle rdf:type owl:ObjectProperty .


###  http://www.semanticweb.org/atb/ontologies/2019/11/PSS-ontology-2#Product_has_ProductFeature
PSS-ontology-2:Product_has_ProductFeature rdf:type owl:ObjectProperty .


###  http://www.semanticweb.org/atb/ontologies/2019/11/PSS-ontology-2#Product_has_ProductLifecycleModel
PSS-ontology-2:Product_has_ProductLifecycleModel rdf:type owl:ObjectProperty .


###  http://www.semanticweb.org/atb/ontologies/2019/11/PSS-ontology-2#Product_has_ProductRole
PSS-ontology-2:Product_has_ProductRole rdf:type owl:ObjectProperty .


###  http://www.semanticweb.org/atb/ontologies/2019/11/PSS-ontology-2#Product_is_composed_of_ProductComponent
PSS-ontology-2:Product_is_composed_of_ProductComponent rdf:type owl:ObjectProperty .


###  http://www.semanticweb.org/atb/ontologies/2019/11/PSS-ontology-2#ServiceComponent_implements_ServiceOfferComponent
PSS-ontology-2:ServiceComponent_implements_ServiceOfferComponent rdf:type owl:ObjectProperty .


###  http://www.semanticweb.org/atb/ontologies/2019/11/PSS-ontology-2#ServiceOfferIntegratedSet_is_composed_of_ServiceOffers
PSS-ontology-2:ServiceOfferIntegratedSet_is_composed_of_ServiceOffers rdf:type owl:ObjectProperty .


###  http://www.semanticweb.org/atb/ontologies/2019/11/PSS-ontology-2#ServiceOffer_has_ServiceLifecycleModel
PSS-ontology-2:ServiceOffer_has_ServiceLifecycleModel rdf:type owl:ObjectProperty .


###  http://www.semanticweb.org/atb/ontologies/2019/11/PSS-ontology-2#ServiceOffer_has_ServiceOfferFeature
PSS-ontology-2:ServiceOffer_has_ServiceOfferFeature rdf:type owl:ObjectProperty .


###  http://www.semanticweb.org/atb/ontologies/2019/11/PSS-ontology-2#ServiceOffer_is_part_of_PSS
PSS-ontology-2:ServiceOffer_is_part_of_PSS rdf:type owl:ObjectProperty .


###  http://www.semanticweb.org/atb/ontologies/2019/11/PSS-ontology-2#ServiceProvider_supplies_Service
PSS-ontology-2:ServiceProvider_supplies_Service rdf:type owl:ObjectProperty .


###  http://www.semanticweb.org/atb/ontologies/2019/11/PSS-ontology-2#Service_exists_in_ServiceLifecycleModel
PSS-ontology-2:Service_exists_in_ServiceLifecycleModel rdf:type owl:ObjectProperty .


###  http://www.semanticweb.org/atb/ontologies/2019/11/PSS-ontology-2#Service_generates_ServiceData
PSS-ontology-2:Service_generates_ServiceData rdf:type owl:ObjectProperty .


###  http://www.semanticweb.org/atb/ontologies/2019/11/PSS-ontology-2#Service_implements_PSS
PSS-ontology-2:Service_implements_PSS rdf:type owl:ObjectProperty .


###  http://www.semanticweb.org/atb/ontologies/2019/11/PSS-ontology-2#Service_implements_ServiceOffer
PSS-ontology-2:Service_implements_ServiceOffer rdf:type owl:ObjectProperty .


###  http://www.semanticweb.org/atb/ontologies/2019/11/PSS-ontology-2#Service_is_composed_of_ServiceComponent
PSS-ontology-2:Service_is_composed_of_ServiceComponent rdf:type owl:ObjectProperty .


###  http://www.semanticweb.org/atb/ontologies/2019/11/PSS-ontology-2#Service_uses_ProductData
PSS-ontology-2:Service_uses_ProductData rdf:type owl:ObjectProperty .


###  http://www.semanticweb.org/atb/ontologies/2019/11/PSS-ontology-2#Service_uses_ServiceData
PSS-ontology-2:Service_uses_ServiceData rdf:type owl:ObjectProperty .


###  http://www.semanticweb.org/atb/ontologies/2019/11/PSS-ontology-2#Stakeholder_defines_Requirements
PSS-ontology-2:Stakeholder_defines_Requirements rdf:type owl:ObjectProperty .


###  http://www.semanticweb.org/atb/ontologies/2019/11/PSS-ontology-2#Stakeholder_provides_Feedback
PSS-ontology-2:Stakeholder_provides_Feedback rdf:type owl:ObjectProperty .


#################################################################
#    Classes
#################################################################

###  http://purl.obolibrary.org/obo/BFO_0000002
obo:BFO_0000002 rdf:type owl:Class .


###  http://purl.obolibrary.org/obo/BFO_0000015
obo:BFO_0000015 rdf:type owl:Class .


###  http://purl.obolibrary.org/obo/BFO_0000017
obo:BFO_0000017 rdf:type owl:Class .


###  http://purl.obolibrary.org/obo/BFO_0000020
obo:BFO_0000020 rdf:type owl:Class .


###  http://purl.obolibrary.org/obo/BFO_0000023
obo:BFO_0000023 rdf:type owl:Class .


###  http://purl.obolibrary.org/obo/BFO_0000031
obo:BFO_0000031 rdf:type owl:Class .


###  http://purl.obolibrary.org/obo/BFO_0000040
obo:BFO_0000040 rdf:type owl:Class .


###  http://purl.obolibrary.org/obo/BFO_0000141
obo:BFO_0000141 rdf:type owl:Class .


###  http://www.semanticweb.org/atb/ontologies/2019/11/PSS-ontology-2#Benefit
PSS-ontology-2:Benefit rdf:type owl:Class ;
                       rdfs:subClassOf PSS-ontology-2:Indicator ;
                       obo:IAO_0000115 "Benefit is an indicator that depicts a positive value (e.g. financial, satisfaction, assistance, etc.)  a stakeholder (e.g. a customer) receives back as a result of the offered PSS." ;
                       dc:contributor "ATB - EPFL" ;
                       rdfs:comment """Examples could be e.g.
cost reduction, eco friendliness, performance improvement, risk reduction.""" ;
                       rdfs:label "benefit" .


###  http://www.semanticweb.org/atb/ontologies/2019/11/PSS-ontology-2#BusinessProcess
PSS-ontology-2:BusinessProcess rdf:type owl:Class ;
                               rdfs:subClassOf obo:BFO_0000015 ;
                               obo:IAO_0000115 "A business process is a planned process that realizes a function of an organization (company/enterprise)." ;
                               dc:contributor "ATB - EPFL" ;
                               rdfs:label "business process" .


###  http://www.semanticweb.org/atb/ontologies/2019/11/PSS-ontology-2#BusinessResource
PSS-ontology-2:BusinessResource rdf:type owl:Class ;
                                rdfs:subClassOf PSS-ontology-2:Resource ;
                                obo:IAO_0000115 "Business resource =def. continuant that bears a business resource role." ;
                                dc:contributor "ATB - EPFL" ;
                                rdfs:label "business resource" .


###  http://www.semanticweb.org/atb/ontologies/2019/11/PSS-ontology-2#BusinessResourceRole
PSS-ontology-2:BusinessResourceRole rdf:type owl:Class ;
                                    rdfs:subClassOf obo:BFO_0000023 ;
                                    obo:IAO_0000115 "business resource role is a role that inheres in an independent continuant where that continuant bears a disposition that, if realized, is realized in a business enterprise process" ;
                                    dc:contributor "ATB - EPFL" ;
                                    rdfs:label "business resource role" .


###  http://www.semanticweb.org/atb/ontologies/2019/11/PSS-ontology-2#Business_Customer
PSS-ontology-2:Business_Customer rdf:type owl:Class ;
                                 rdfs:subClassOf PSS-ontology-2:Company ;
                                 obo:IAO_0000115 "Business Customer is a Company that buys and uses the products, services or PSS. It is the (group/company) customer of the PSS, using the PSS for their own business." ;
                                 dc:contributor "ATB - EPFL" ;
                                 rdfs:label "Business Customer" .


###  http://www.semanticweb.org/atb/ontologies/2019/11/PSS-ontology-2#Business_Model
PSS-ontology-2:Business_Model rdf:type owl:Class ;
                              rdfs:subClassOf obo:BFO_0000020 ;
                              obo:IAO_0000115 "Business Model is a description of a plan and implementation of the plan, aiming the successful operation of a business." ;
                              dc:contributor "ATB - EPFL" ;
                              rdfs:comment "This is an interface class to other ontologies." ;
                              rdfs:label "Business Model" .


###  http://www.semanticweb.org/atb/ontologies/2019/11/PSS-ontology-2#Company
PSS-ontology-2:Company rdf:type owl:Class ;
                       rdfs:subClassOf <http://www.semanticweb.org/atb/ontologies/2019/11/PSS-ontology-2#Stakeholder/Actor> ;
                       obo:IAO_0000115 "Company is a Stakeholder that can be one or more individuals forming a legal entity (corporate body)." ;
                       dc:contributor "ATB - EPFL" ;
                       rdfs:label "Company" .


###  http://www.semanticweb.org/atb/ontologies/2019/11/PSS-ontology-2#Data
PSS-ontology-2:Data rdf:type owl:Class ;
                    rdfs:subClassOf PSS-ontology-2:Resource ;
                    obo:IAO_0000115 "PSS Source-Data is a Resource that refers to the digitalised information coming as input from the product or the service, specifically for the scope of PSS." ;
                    dc:contributor "ATB - EPFL" ;
                    rdfs:label "PSS Source-Data" .


###  http://www.semanticweb.org/atb/ontologies/2019/11/PSS-ontology-2#Embedded_Data
PSS-ontology-2:Embedded_Data rdf:type owl:Class ;
                             rdfs:subClassOf PSS-ontology-2:Product_Data ;
                             obo:IAO_0000115 "Embedded Data are Product Data generated from embedded data-source components (e.g. sensors)." ;
                             dc:contributor "ATB - EPFL" ;
                             rdfs:label "Embedded Data" .


###  http://www.semanticweb.org/atb/ontologies/2019/11/PSS-ontology-2#Embedded_Data_Source_Component
PSS-ontology-2:Embedded_Data_Source_Component rdf:type owl:Class ;
                                              rdfs:subClassOf PSS-ontology-2:Product_Component ;
                                              obo:IAO_0000115 "Embedded Data-Source Component is a Product Component that refers to product-embedded information devices / parts (e.g. sensors), which allows for (additional) services to be offered for the product." ;
                                              dc:contributor "ATB - EPFL" ;
                                              rdfs:label "Embedded Data-Source Component" .


###  http://www.semanticweb.org/atb/ontologies/2019/11/PSS-ontology-2#Employee
PSS-ontology-2:Employee rdf:type owl:Class ;
                        rdfs:subClassOf PSS-ontology-2:Individual_Person ;
                        obo:IAO_0000115 "Employee is an Individual Person that works in a Company (PSS-related company)." ;
                        dc:contributor "ATB - EPFL" ;
                        rdfs:label "Employee" .


###  http://www.semanticweb.org/atb/ontologies/2019/11/PSS-ontology-2#Feature
PSS-ontology-2:Feature rdf:type owl:Class ;
                       rdfs:subClassOf PSS-ontology-2:Information ;
                       obo:IAO_0000115 "Feature is PSS Information that describes the characteristics of a product, service, or PSS." ;
                       dc:contributor "ATB - EPFL" .


###  http://www.semanticweb.org/atb/ontologies/2019/11/PSS-ontology-2#Feedback
PSS-ontology-2:Feedback rdf:type owl:Class ;
                        rdfs:subClassOf PSS-ontology-2:Information ;
                        obo:IAO_0000115 "Feedback is PSS Information that represents any opinion on PSS, product or service (e.g. comments on social media, opinion expression in online questionnaires, etc.), coming from the Stakeholders (e.g., Business or Individual Customers)." ;
                        dc:contributor "ATB - EPFL" ;
                        rdfs:label "feedback" .


###  http://www.semanticweb.org/atb/ontologies/2019/11/PSS-ontology-2#Firmware
PSS-ontology-2:Firmware rdf:type owl:Class ;
                        rdfs:subClassOf PSS-ontology-2:Product_Component ;
                        obo:IAO_0000115 "Firmware is a Product Component which is software, i.e. control software of a machine that exists only in combination with specific hardware product." ;
                        dc:contributor "ATB - EPFL" .


###  http://www.semanticweb.org/atb/ontologies/2019/11/PSS-ontology-2#Guideline
PSS-ontology-2:Guideline rdf:type owl:Class ;
                         rdfs:subClassOf PSS-ontology-2:Information ;
                         obo:IAO_0000115 "Guideline is PSS Information referring to a statement describing a course of action aiming to reach a specific goal for the design, development or use of a PSS." ;
                         dc:contributor "ATB - EPFL" ;
                         rdfs:label "guideline" .


###  http://www.semanticweb.org/atb/ontologies/2019/11/PSS-ontology-2#Hardware_Infrastructure
PSS-ontology-2:Hardware_Infrastructure rdf:type owl:Class ;
                                       rdfs:subClassOf PSS-ontology-2:Infrastructure ;
                                       obo:IAO_0000115 "Hardware Infrastructure is an Infrastructure that refers to the physical networks (resources) necessary for the design, development, delivery and operation of the PSS." ;
                                       dc:contributor "ATB - EPFL" ;
                                       rdfs:label "hardware infrastucture" .


###  http://www.semanticweb.org/atb/ontologies/2019/11/PSS-ontology-2#Indicator
PSS-ontology-2:Indicator rdf:type owl:Class ;
                         rdfs:subClassOf PSS-ontology-2:Information ;
                         obo:IAO_0000115 "Indicator is PSS Information used to measure/evaluate any aspect within the scope of PSS, namely a process, a PSS, a product, a service, etc." ;
                         dc:contributor "ATB - EPFL" ;
                         rdfs:label "indicator" .


###  http://www.semanticweb.org/atb/ontologies/2019/11/PSS-ontology-2#Individual_Customer
PSS-ontology-2:Individual_Customer rdf:type owl:Class ;
                                   rdfs:subClassOf PSS-ontology-2:Individual_Person ;
                                   obo:IAO_0000115 "Individual Customer (Consumer) is an Individual Person that buys or consumes (consumer) any product/service in the PSS." ;
                                   dc:contributor "ATB - EPFL" ;
                                   rdfs:label "Individual Customer (Consumer)" .


###  http://www.semanticweb.org/atb/ontologies/2019/11/PSS-ontology-2#Individual_Person
PSS-ontology-2:Individual_Person rdf:type owl:Class ;
                                 rdfs:subClassOf <http://www.semanticweb.org/atb/ontologies/2019/11/PSS-ontology-2#Stakeholder/Actor> ;
                                 obo:IAO_0000115 "Individual Person is a Stakeholder indicating a separate person who is not legal entity (i.e. not legally considered a corporate group, as for example a company)." ;
                                 dc:contributor "ATB - EPFL" ;
                                 rdfs:label "Individual Person" .


###  http://www.semanticweb.org/atb/ontologies/2019/11/PSS-ontology-2#Information
PSS-ontology-2:Information rdf:type owl:Class ;
                           rdfs:subClassOf PSS-ontology-2:Resource ;
                           obo:IAO_0000115 "PSS Information is a Resource, immaterial, describing aspects affecting PSS, and referring to all the (processed) data that one can acquire knowledge from, or further process." ;
                           dc:contributor "ATB - EPFL" ;
                           rdfs:comment "Name to be changed to Immaterial Resources?" ;
                           rdfs:label "PSS Information" .


###  http://www.semanticweb.org/atb/ontologies/2019/11/PSS-ontology-2#Infrastructure
PSS-ontology-2:Infrastructure rdf:type owl:Class ;
                              rdfs:subClassOf PSS-ontology-2:Resource ;
                              obo:IAO_0000115 "Infrastructure is a Resource describing the facilities (physical e.g. buildings or machines, and organisational e.g. computer networks or software applications) used to assist in development and delivering of the PSS." ;
                              obo:IAO_0000118 "Infrastructure is a Material Resource including the physical (e.g. buildings or machines, computers), and organisational (e.g. communication networks) means used to assist in development and delivering of the Product and Services." ;
                              dc:contributor "ATB - EPFL" ;
                              rdfs:comment "It may serve as an interface class for merging with other ontologies." ;
                              rdfs:label "infrastructure" .


###  http://www.semanticweb.org/atb/ontologies/2019/11/PSS-ontology-2#KPI
PSS-ontology-2:KPI rdf:type owl:Class ;
                   rdfs:subClassOf PSS-ontology-2:Indicator ;
                   obo:IAO_0000115 "Key Performance Indicator (KPI) is an Indicator referring to (a set of) measurement(s) that evaluates the performance (or success) of a PSS (concept), and is business relevant." ;
                   dc:contributor "ATB - EPFL" ;
                   rdfs:comment """Various types of KPIs can be defined: manufacturing KPI, environmental KPI etc. 
This is an interface class to other ontologies""" .


###  http://www.semanticweb.org/atb/ontologies/2019/11/PSS-ontology-2#Lifecycle
PSS-ontology-2:Lifecycle rdf:type owl:Class ;
                         rdfs:subClassOf obo:BFO_0000015 ;
                         obo:IAO_0000115 "Lifecycle is a set of Processes the PSS, a product or a service uses for its activities from the idea conceptualisation to its end-of-life. It refers to the Lifecycle Model entity in conjunction with time." ;
                         dc:contributor "ATB - EPFL" ;
                         rdfs:comment "This is an interface class to other ontologies." ;
                         rdfs:label "Lifecycle" .


###  http://www.semanticweb.org/atb/ontologies/2019/11/PSS-ontology-2#Lifecycle_Model
PSS-ontology-2:Lifecycle_Model rdf:type owl:Class ;
                               rdfs:subClassOf obo:BFO_0000017 ;
                               obo:IAO_0000115 "Lifecycle Model is a (set of) Process Definition(s) which includes different activities in the life of PSS, product, service etc. from the idea conceptualisation to its end-of life (beginning-of -life, middle-of-life, end-of-life)." ;
                               dc:contributor "ATB - EPFL" ;
                               rdfs:comment "This is an interface class to other ontologies." ;
                               rdfs:label "Lifecycle Model" .


###  http://www.semanticweb.org/atb/ontologies/2019/11/PSS-ontology-2#ManufacturingEnterpriseProcess
PSS-ontology-2:ManufacturingEnterpriseProcess rdf:type owl:Class ;
                                              rdfs:subClassOf obo:BFO_0000015 ;
                                              obo:IAO_0000115 "Manufacturing enterprise process=def. planned process that has agent some manufacturing enterprise, where the agent realizes the planned processes of the enterprise." ;
                                              dc:contributor "ATB - EPFL" ;
                                              rdfs:label "manufacturing enterprise process" .


###  http://www.semanticweb.org/atb/ontologies/2019/11/PSS-ontology-2#ManufacturingResource
PSS-ontology-2:ManufacturingResource rdf:type owl:Class ;
                                     rdfs:subClassOf PSS-ontology-2:Resource ;
                                     obo:IAO_0000115 "IOF: Manufacturing resource =def. continuant that bears a manufacturing resource role." ;
                                     dc:contributor "ATB - EPFL" ;
                                     rdfs:label "manufacturing resource" .


###  http://www.semanticweb.org/atb/ontologies/2019/11/PSS-ontology-2#ManufacturingResourceRole
PSS-ontology-2:ManufacturingResourceRole rdf:type owl:Class ;
                                         rdfs:subClassOf obo:BFO_0000023 ;
                                         obo:IAO_0000115 "Is a role that inheres in an independent continuant where that continuant bears a disposition that, if realized, is realized in a manufacturing enterprise process" ;
                                         rdfs:label "manufacturing resource role" .


###  http://www.semanticweb.org/atb/ontologies/2019/11/PSS-ontology-2#Material_Object
PSS-ontology-2:Material_Object rdf:type owl:Class ;
                               rdfs:subClassOf obo:BFO_0000002 ;
                               obo:IAO_0000115 "Material Object is a group describing manufactured physical/material entities." ;
                               dc:contributor "ATB - EPFL" ;
                               rdfs:label "Material Object" .


###  http://www.semanticweb.org/atb/ontologies/2019/11/PSS-ontology-2#PSS
PSS-ontology-2:PSS rdf:type owl:Class ;
                   rdfs:subClassOf PSS-ontology-2:System ;
                   obo:IAO_0000115 "Product Service System (PSS) is a System that aims to satisfy a need of the market (e.g. to be sold in order to provide profit and support customers by covering their needs), to be competitive, and jointly fulfil customer’s needs [3]. It must include products and services, and may include stakeholders and infrastructure (software or hardware)." ;
                   obo:IAO_0000118 "PSS is a system which includes at least one product and at least one service, related to this product, and may include stakeholders and infrastructure and which bears PSS Role." ,
                                   """PSS is a system which includes at least one product and at least one service, related to this product, and which bears PSS Role.
PSS role is a role that borne by set of at least an entity that is the specified output of a product production process and at least an entity that is the specified output of a service development process""" ;
                   obo:IAO_0000119 """Resources:

3. Mont, Oksana K. \"Clarifying the concept of product–service system.\" Journal of cleaner production 10.3 (2002): 237-245.""" ;
                   dc:contributor "ATB - EPFL" ;
                   rdfs:comment "This is an interface class to other ontologies." ;
                   rdfs:label "PSS" .


###  http://www.semanticweb.org/atb/ontologies/2019/11/PSS-ontology-2#PSS-Development_Condition
PSS-ontology-2:PSS-Development_Condition rdf:type owl:Class ;
                                         rdfs:subClassOf PSS-ontology-2:PSS_Condition ;
                                         obo:IAO_0000115 "PSS-Development Condition is a PSS Condition which describes the situation under which the PSS is being developed (e.g. cultural characteristics of the development teams, corporate orientation preferences, etc.)" ;
                                         dc:contributor "ATB - EPFL" ;
                                         rdfs:comment "It may serve as an interface class for merging with other ontologies (e.g. in DIVERSITY to user-centric ontology [7])." ;
                                         rdfs:label "PSS-Development Condition" .


###  http://www.semanticweb.org/atb/ontologies/2019/11/PSS-ontology-2#PSS-Use_Condition
PSS-ontology-2:PSS-Use_Condition rdf:type owl:Class ;
                                 rdfs:subClassOf PSS-ontology-2:PSS_Condition ;
                                 obo:IAO_0000115 "PSS-Use Condition is a PSS Condition which describes the situation under which the PSS is being used (e.g. environment aspects, cultural aspect, geographical location, etc.)." ;
                                 dc:contributor "ATB - EPFL" ;
                                 rdfs:comment "It may serve as an interface class for merging with other ontologies." ;
                                 rdfs:label "PSS-Use Condition" .


###  http://www.semanticweb.org/atb/ontologies/2019/11/PSS-ontology-2#PSSBusinessProcess
PSS-ontology-2:PSSBusinessProcess rdf:type owl:Class ;
                                  rdfs:subClassOf obo:BFO_0000015 ;
                                  obo:IAO_0000115 "PSS Business Process is a process in which PSS is developed, implemented, distributed and used." ;
                                  obo:IAO_0000118 "A PSS business process is a planned process that realizes a function which is related to generation of a system which bears a PSS role" ;
                                  dc:contributor "ATB - EPFL" ;
                                  rdfs:label "PSS business process" .


###  http://www.semanticweb.org/atb/ontologies/2019/11/PSS-ontology-2#PSS_Condition
PSS-ontology-2:PSS_Condition rdf:type owl:Class ;
                             rdfs:subClassOf obo:BFO_0000141 ;
                             obo:IAO_0000115 "PSS Condition is a non-material entity that describes the situation around PSS." ;
                             dc:contributor "ATB - EPFL" ;
                             rdfs:label "PSS Condition" .


###  http://www.semanticweb.org/atb/ontologies/2019/11/PSS-ontology-2#PSS_Feature
PSS-ontology-2:PSS_Feature rdf:type owl:Class ;
                           rdfs:subClassOf PSS-ontology-2:Feature ;
                           obo:IAO_0000115 "PSS Feature is a Feature that describes an aspect or attribute related to the PSS." ;
                           dc:contributor "ATB - EPFL" ;
                           rdfs:label "PSS Feature" .


###  http://www.semanticweb.org/atb/ontologies/2019/11/PSS-ontology-2#PSS_Lifecycle
PSS-ontology-2:PSS_Lifecycle rdf:type owl:Class ;
                             rdfs:subClassOf PSS-ontology-2:Lifecycle ;
                             obo:IAO_0000115 "PSS Lifecycle is a Lifecycle that includes the PSS processes from the idea conceptualisation to its end-of-life, referring to the PSS Lifecycle Model in conjunction with time." ;
                             dc:contributor "ATB - EPFL" ;
                             rdfs:label "PSS Lifecycle" .


###  http://www.semanticweb.org/atb/ontologies/2019/11/PSS-ontology-2#PSS_Lifecycle_Model
PSS-ontology-2:PSS_Lifecycle_Model rdf:type owl:Class ;
                                   rdfs:subClassOf PSS-ontology-2:Lifecycle_Model ;
                                   obo:IAO_0000115 "PSS Lifecycle Model is the Lifecycle Model that refers to the different stages of the life of PSS." ;
                                   dc:contributor "ATB - EPFL" ;
                                   rdfs:label "PSS Lifecycle Model" .


###  http://www.semanticweb.org/atb/ontologies/2019/11/PSS-ontology-2#PSS_Provider
PSS-ontology-2:PSS_Provider rdf:type owl:Class ;
                            rdfs:subClassOf <http://www.semanticweb.org/atb/ontologies/2019/11/PSS-ontology-2#Supplier/Provider/Vendor> ;
                            obo:IAO_0000115 "PSS Provider is a Supplier/ Provider/Vendor that offers PSS and owns intellectual property rights (IPR) on PSS offer." ;
                            dc:contributor "ATB - EPFL" ;
                            rdfs:label "PSS Provider" .


###  http://www.semanticweb.org/atb/ontologies/2019/11/PSS-ontology-2#PSS_Role
PSS-ontology-2:PSS_Role rdf:type owl:Class ;
                        rdfs:subClassOf obo:BFO_0000023 ;
                        obo:IAO_0000115 "PSS role is a role that borne by set of at least an entity that is the specified output of a product production process and at least an entity that is the specified output of a service development process, and may include material entity that is used in PSS processes and actors that are involved in PSS processes. This set is intended to satisfy a need of the market, to be competitive, and jointly fulfil customer’s needs." ;
                        obo:IAO_0000118 "PSS role is a role that borne by set of at least an entity that is the specified output of a product production process and at least an entity that is the specified output of a service development process." ;
                        dc:contributor "ATB - EPFL" ;
                        rdfs:comment "PSS Role is an optional characteristic of a system combining products and services, aiming to satisfy a need of the market (e.g. to be sold in order to provide profit and support customers by covering their needs)." ;
                        rdfs:label "PSS Role" .


###  http://www.semanticweb.org/atb/ontologies/2019/11/PSS-ontology-2#PSS_Type
PSS-ontology-2:PSS_Type rdf:type owl:Class ;
                        rdfs:subClassOf PSS-ontology-2:PSS_Feature ;
                        obo:IAO_0000112 "Typical examples of PSS with a different type feature are e.g. the product- oriented PSS, the result-oriented PSS and the use-oriented PSS." ;
                        obo:IAO_0000115 "PSS-Type Feature is a PSS Feature that refers to characteristics that define the subgroup where a PSS belongs to, and describe the specific focus (orientation or aim) of a PSS, such as to engage the customer with services, or to increase the sales of a product." ;
                        dc:contributor "ATB - EPFL" ;
                        rdfs:label "PSS Type Feature" .


###  http://www.semanticweb.org/atb/ontologies/2019/11/PSS-ontology-2#Process_Definition
PSS-ontology-2:Process_Definition rdf:type owl:Class ;
                                  rdfs:subClassOf obo:BFO_0000017 ;
                                  obo:IAO_0000115 "Process Definition is a structured set of activities designed to accomplish a specific objective [4]. For example, the Process Definition can be the manufacturing process where the equipment is manufactured, or the process where the equipment is used, or the development process where products, services or PSS are being developed etc." ;
                                  obo:IAO_0000119 """Resources:

4. Wikipedia contributors, 'Business process', Wikipedia, The Free Encyclopaedia, 17 July 2017, 11:25 UTC, <https://en.wikipedia.org/w/index.php?title=Business_process&oldid=790986805> [accessed 20 July 2017]""" ;
                                  dc:contributor "ATB - EPFL" ;
                                  rdfs:comment "NOTE: Relation to BFO - Under continuant the process (definition) is being modelled as part of the PSS environment without including the time duration in which this process is valid. The time aspect of the process is included, however, as part of the modelling as occurrent." ;
                                  rdfs:label "Process Definition" .


###  http://www.semanticweb.org/atb/ontologies/2019/11/PSS-ontology-2#Product
PSS-ontology-2:Product rdf:type owl:Class ;
                       rdfs:subClassOf PSS-ontology-2:Material_Object ;
                       obo:IAO_0000115 "Product (for manufacturing industry) is a Material Object, manufactured to satisfy a need of the market [5] (e.g. to be sold in order to provide profit and support customers by covering their needs)." ;
                       obo:IAO_0000118 "A PSS:product is a commercially distributed good that is a tangible property and (1) the output of a fabrication, manufacturing, or production process, and (2) something that passes through a distribution channel before being consumed or used'" ,
                                       "A Product is an entity that bears a product role" ;
                       obo:IAO_0000119 "5. Wikipedia contributors, 'Product', Wikipedia, The Free Encyclopaedia, 10 July 2017, 15:21 UTC, <https://en.wikipedia.org/w/index.php?title=Product&oldid=789934020> [accessed 20 July 2017]" ;
                       dc:contributor "ATB - EPFL" ;
                       rdfs:comment "It may serve as an interface class for merging with other ontologies." ;
                       rdfs:label "product" .


###  http://www.semanticweb.org/atb/ontologies/2019/11/PSS-ontology-2#ProductProductionProcess
PSS-ontology-2:ProductProductionProcess rdf:type owl:Class ;
                                        rdfs:subClassOf obo:BFO_0000015 ;
                                        dc:contributor "A product production process is a planned process that has output some continuant, where the continuant did not exist prior to the planned process, and where the agent who performs the process intends for the continuant to bear a product role." ,
                                                       "ATB - EPFL" ;
                                        rdfs:label "product production process" .


###  http://www.semanticweb.org/atb/ontologies/2019/11/PSS-ontology-2#Product_Component
PSS-ontology-2:Product_Component rdf:type owl:Class ;
                                 rdfs:subClassOf PSS-ontology-2:Material_Object ;
                                 obo:IAO_0000115 "Product Component is a Material Object which is part of the Product. It can be itself a manufactured product, but for the offered product within the scope of PSS, its existence only has a meaning as part of the product." ;
                                 dc:contributor "ATB - EPFL" ;
                                 rdfs:comment "It may serve as an interface class for merging with other ontologies." ;
                                 rdfs:label "Product Component" .


###  http://www.semanticweb.org/atb/ontologies/2019/11/PSS-ontology-2#Product_Data
PSS-ontology-2:Product_Data rdf:type owl:Class ;
                            rdfs:subClassOf PSS-ontology-2:Data ;
                            obo:IAO_0000115 "Product Data are PSS Source-Data used in the scope of PSS, and refer specifically to the product part of PSS." ;
                            dc:contributor "ATB - EPFL" ;
                            rdfs:label "Product Data" .


###  http://www.semanticweb.org/atb/ontologies/2019/11/PSS-ontology-2#Product_Extension_Service
PSS-ontology-2:Product_Extension_Service rdf:type owl:Class ;
                                         rdfs:subClassOf PSS-ontology-2:Service ;
                                         obo:IAO_0000115 "Product Extension Service is a Service which adds additional value to the product." ;
                                         dc:contributor "ATB - EPFL" ;
                                         rdfs:label "Product Extension Service" .


###  http://www.semanticweb.org/atb/ontologies/2019/11/PSS-ontology-2#Product_Extension_Service_Offer
PSS-ontology-2:Product_Extension_Service_Offer rdf:type owl:Class ;
                                               rdfs:subClassOf PSS-ontology-2:Service_Offer ;
                                               obo:IAO_0000115 "Product-Extension Service-Offer is a Service Offer which adds value to the product." ;
                                               dc:contributor "ATB - EPFL" ;
                                               rdfs:label "Product Extension Service Offer" .


###  http://www.semanticweb.org/atb/ontologies/2019/11/PSS-ontology-2#Product_Feature
PSS-ontology-2:Product_Feature rdf:type owl:Class ;
                               rdfs:subClassOf PSS-ontology-2:Feature ;
                               obo:IAO_0000115 "Product Feature is a Feature that describes an aspect, or attribute, related to the product within the PSS scope." ;
                               dc:contributor "ATB - EPFL" ;
                               rdfs:label "Product Feature" .


###  http://www.semanticweb.org/atb/ontologies/2019/11/PSS-ontology-2#Product_Integrated_Set
PSS-ontology-2:Product_Integrated_Set rdf:type owl:Class ;
                                      rdfs:subClassOf PSS-ontology-2:Material_Object ;
                                      obo:IAO_0000115 "Product Integrated Set is a Material Object that consists of a set of products needed to jointly fulfil users’ needs." ;
                                      dc:contributor "ATB - EPFL" ;
                                      rdfs:label "Product Integrated Set" .


###  http://www.semanticweb.org/atb/ontologies/2019/11/PSS-ontology-2#Product_Lifecycle
PSS-ontology-2:Product_Lifecycle rdf:type owl:Class ;
                                 rdfs:subClassOf PSS-ontology-2:Lifecycle ;
                                 obo:IAO_0000115 "Product Lifecycle is a Lifecycle that includes only the Product-specific processes, in the scope of PSS. It refers to the Product Lifecycle Model in conjunction with time." ;
                                 dc:contributor "ATB - EPFL" ;
                                 rdfs:label "Product Lifecycle" .


###  http://www.semanticweb.org/atb/ontologies/2019/11/PSS-ontology-2#Product_Lifecycle_Model
PSS-ontology-2:Product_Lifecycle_Model rdf:type owl:Class ;
                                       rdfs:subClassOf PSS-ontology-2:Lifecycle_Model ;
                                       obo:IAO_0000115 "Product Lifecycle Model is a Lifecycle Model that refers to the product within the scope of PSS." ;
                                       dc:contributor "ATB - EPFL" ;
                                       rdfs:label "Product Lifecycle Model" .


###  http://www.semanticweb.org/atb/ontologies/2019/11/PSS-ontology-2#Product_Provider
PSS-ontology-2:Product_Provider rdf:type owl:Class ;
                                rdfs:subClassOf <http://www.semanticweb.org/atb/ontologies/2019/11/PSS-ontology-2#Supplier/Provider/Vendor> ;
                                obo:IAO_0000115 "Product Provider is a Supplier/ provider/vendor that both produces and sells a product, or only sells it." ;
                                dc:contributor "ATB - EPFL" ;
                                rdfs:label "Product Provider" .


###  http://www.semanticweb.org/atb/ontologies/2019/11/PSS-ontology-2#Product_Role
PSS-ontology-2:Product_Role rdf:type owl:Class ;
                            rdfs:subClassOf obo:BFO_0000023 ;
                            obo:IAO_0000115 "A Product Role is a role borne by an entity that is the specified output of a product production process" ;
                            obo:IAO_0000118 "A Product Role is a role borne by an entity that is the specified output of a product production process Role that is borne by a BFO: Continuant intended to be sold (and bearing some economic value, the value can be zero, positive, or negative)" ,
                                            "Product Role is an optional characteristic of a material object manufactured to satisfy a need of the market (e.g. to be sold in order to provide profit and support customers by covering their needs)." ;
                            dc:contributor "ATB - EPFL" ;
                            rdfs:label "product role" .


###  http://www.semanticweb.org/atb/ontologies/2019/11/PSS-ontology-2#Product_Type_Feature
PSS-ontology-2:Product_Type_Feature rdf:type owl:Class ;
                                    rdfs:subClassOf PSS-ontology-2:Product_Feature ;
                                    obo:IAO_0000115 "Product-Type Feature is a Product Feature that refers to characteristics that define the subgroup where a product belongs to." ;
                                    dc:contributor "ATB - EPFL" ;
                                    rdfs:comment "Product type is sector or company specific. These are features which characterise the specific type (subgroup) of the product." ;
                                    rdfs:label "Product Type Feature" .


###  http://www.semanticweb.org/atb/ontologies/2019/11/PSS-ontology-2#Requirement
PSS-ontology-2:Requirement rdf:type owl:Class ;
                           rdfs:subClassOf PSS-ontology-2:Information ;
                           obo:IAO_0000115 "Requirement is PSS Information that depicts the aspects which are necessary for the design, development or offer of PSS. Requirement is defined by the Stakeholder." ;
                           dc:contributor "ATB - EPFL" ;
                           rdfs:comment """Requirement can be further extended according to the ISO standard or other System Engineering references.
Here it serves as an interface class for merging with other ontologies.""" .


###  http://www.semanticweb.org/atb/ontologies/2019/11/PSS-ontology-2#Resource
PSS-ontology-2:Resource rdf:type owl:Class ;
                        rdfs:subClassOf obo:BFO_0000031 ;
                        obo:IAO_0000115 "Resource is a mean (source) that can be used for the design, development, offer and delivery of a PSS, from which benefit can be produced [2]." ;
                        obo:IAO_0000119 """Resources:

2.  Wikipedia contributors, 'Resource', Wikipedia, The Free Encyclopaedia, 27 June 2017, 08:20 UTC, <https://en.wikipedia.org/w/index.php?title=Resource&oldid=787741678> [accessed 20 July 2017]""" ;
                        dc:contributor "ATB - EPFL" ;
                        rdfs:label "resource" .


###  http://www.semanticweb.org/atb/ontologies/2019/11/PSS-ontology-2#Service
PSS-ontology-2:Service rdf:type owl:Class ;
                       rdfs:subClassOf obo:BFO_0000015 ;
                       obo:IAO_0000115 "Service is a Process made for, and driven by customers, with economic value, and refers to the Service Offer entity in conjunction with time." ;
                       dc:contributor "ATB - EPFL" ;
                       rdfs:comment "This is an interface class to other ontologies." .


###  http://www.semanticweb.org/atb/ontologies/2019/11/PSS-ontology-2#ServiceResource
PSS-ontology-2:ServiceResource rdf:type owl:Class ;
                               rdfs:subClassOf obo:BFO_0000031 ;
                               obo:IAO_0000115 "Service resource =def. continuant that bears a service resource role." ;
                               rdfs:label "service resource" .


###  http://www.semanticweb.org/atb/ontologies/2019/11/PSS-ontology-2#ServiceResourceRole
PSS-ontology-2:ServiceResourceRole rdf:type owl:Class ;
                                   rdfs:subClassOf obo:BFO_0000023 ;
                                   obo:IAO_0000115 "Role that inheres in an independent continuant where that continuant bears a disposition that, if realized, is realized in a service development and deployment/use processes" ;
                                   dc:contributor "ATB - EPFL" ;
                                   rdfs:label "service resource role" .


###  http://www.semanticweb.org/atb/ontologies/2019/11/PSS-ontology-2#Service_Component
PSS-ontology-2:Service_Component rdf:type owl:Class ;
                                 rdfs:subClassOf obo:BFO_0000015 ;
                                 obo:IAO_0000115 "Service Component is a Process, part of a Service, and refers to the Service Offer Component in conjunction with time." ;
                                 dc:contributor "ATB - EPFL" ;
                                 rdfs:label "Service Component" .


###  http://www.semanticweb.org/atb/ontologies/2019/11/PSS-ontology-2#Service_Data
PSS-ontology-2:Service_Data rdf:type owl:Class ;
                            rdfs:subClassOf PSS-ontology-2:Data ;
                            obo:IAO_0000115 "Service Data are PSS Source Data used in the scope of PSS, and are generated specifically in the service part of PSS (e.g. data generated during a call in the service centre)." ;
                            dc:contributor "ATB - EPFL" ;
                            rdfs:label "Service Data" .


###  http://www.semanticweb.org/atb/ontologies/2019/11/PSS-ontology-2#Service_Feature
PSS-ontology-2:Service_Feature rdf:type owl:Class ;
                               rdfs:subClassOf PSS-ontology-2:Feature ;
                               obo:IAO_0000115 "Service-Offer Feature is a Feature that describes an aspect or attribute related to the service within the PSS scope." ;
                               dc:contributor "ATB - EPFL" ;
                               rdfs:label "Service Offer Feature" .


###  http://www.semanticweb.org/atb/ontologies/2019/11/PSS-ontology-2#Service_Lifecycle
PSS-ontology-2:Service_Lifecycle rdf:type owl:Class ;
                                 rdfs:subClassOf PSS-ontology-2:Lifecycle ;
                                 obo:IAO_0000115 "Service Lifecycle is a Lifecycle that includes only the service-specific processes, in the scope of PSS. It refers to the Service Lifecycle Model in conjunction with time." ;
                                 dc:contributor "ATB - EPFL" ;
                                 rdfs:label "Service Lifecycle" .


###  http://www.semanticweb.org/atb/ontologies/2019/11/PSS-ontology-2#Service_Lifecycle_Model
PSS-ontology-2:Service_Lifecycle_Model rdf:type owl:Class ;
                                       rdfs:subClassOf PSS-ontology-2:Lifecycle_Model ;
                                       obo:IAO_0000115 "Service Lifecycle Model is the Lifecycle Model that refers to the Service Offer within the scope of PSS." ;
                                       dc:contributor "ATB - EPFL" ;
                                       rdfs:label "Service Lifecycle Model" .


###  http://www.semanticweb.org/atb/ontologies/2019/11/PSS-ontology-2#Service_Offer
PSS-ontology-2:Service_Offer rdf:type owl:Class ;
                             rdfs:subClassOf PSS-ontology-2:Process_Definition ;
                             obo:IAO_0000115 "Service Offer is a Process Definition referring to a set of non-tangible entities (activities, software modules etc.), related to the service part of PSS, which aims to satisfy a need of the market (e.g. to be sold in order to provide profit and support customers by covering their needs)." ;
                             obo:IAO_0000118 "Service Offer is a description/definition of a Service (all the activities that have to be done to fulfil the Service)" ;
                             dc:contributor "ATB - EPFL" ;
                             rdfs:comment "This is an interface class to other ontologies." ;
                             rdfs:label "Service Offer" .


###  http://www.semanticweb.org/atb/ontologies/2019/11/PSS-ontology-2#Service_Offer_Component
PSS-ontology-2:Service_Offer_Component rdf:type owl:Class ;
                                       rdfs:subClassOf PSS-ontology-2:Process_Definition ;
                                       obo:IAO_0000115 "Service-Offer Component is a Process Definition which is part of a Service Offer. It can be itself a service, but for the offered service within the scope of PSS, its existence only has a meaning as part of the PSS service offer." ;
                                       dc:contributor "ATB - EPFL" ;
                                       rdfs:label "Service Offer Component" .


###  http://www.semanticweb.org/atb/ontologies/2019/11/PSS-ontology-2#Service_Offer_Integrated_set
PSS-ontology-2:Service_Offer_Integrated_set rdf:type owl:Class ;
                                            rdfs:subClassOf PSS-ontology-2:Process_Definition ;
                                            obo:IAO_0000115 "Service Offer Integrated-Set is a Process Definition that refers to a set of Service Offers, needed to jointly fulfil users’ needs." ;
                                            dc:contributor "ATB - EPFL" ;
                                            rdfs:label "Service Offer Integrated Set" .


###  http://www.semanticweb.org/atb/ontologies/2019/11/PSS-ontology-2#Service_Offer_Role
PSS-ontology-2:Service_Offer_Role rdf:type owl:Class ;
                                  rdfs:subClassOf obo:BFO_0000023 ;
                                  obo:IAO_0000115 "Service Offer Role is an optional characteristic of a non-tangible entity that aims to satisfy a need of the market (e.g. to be sold in order to provide profit and support customers by covering their needs)." ;
                                  obo:IAO_0000118 "A service offer role is a role borne by an entity that is the specified output of a service offer development process" ;
                                  dc:contributor "ATB - EPFL" ;
                                  rdfs:label "service offer role" .


###  http://www.semanticweb.org/atb/ontologies/2019/11/PSS-ontology-2#Service_Provider
PSS-ontology-2:Service_Provider rdf:type owl:Class ;
                                rdfs:subClassOf <http://www.semanticweb.org/atb/ontologies/2019/11/PSS-ontology-2#Supplier/Provider/Vendor> ;
                                obo:IAO_0000115 "Service Provider is a Supplier/ provider/vendor that offers a service." ;
                                dc:contributor "ATB - EPFL" ;
                                rdfs:label "Service Provider" .


###  http://www.semanticweb.org/atb/ontologies/2019/11/PSS-ontology-2#Service_Type_Feature
PSS-ontology-2:Service_Type_Feature rdf:type owl:Class ;
                                    rdfs:subClassOf PSS-ontology-2:Service_Feature ;
                                    obo:IAO_0000115 "Service-Type Feature is a Service Feature that refers to characteristics that define the subgroup where a service belongs to." ;
                                    dc:contributor "ATB - EPFL" ;
                                    rdfs:comment "Service type is sectorial or company specific" ;
                                    rdfs:label "Service Type Feature" .


###  http://www.semanticweb.org/atb/ontologies/2019/11/PSS-ontology-2#Software_Infrastructure
PSS-ontology-2:Software_Infrastructure rdf:type owl:Class ;
                                       rdfs:subClassOf PSS-ontology-2:Infrastructure ;
                                       obo:IAO_0000115 "Software is an infrastructure that refers to the non-material aspects (resources) necessary for the design, development, delivery and operation of the PSS." ;
                                       dc:contributor "ATB - EPFL" ;
                                       rdfs:label "software infrastucture" .


###  http://www.semanticweb.org/atb/ontologies/2019/11/PSS-ontology-2#Software_Log
PSS-ontology-2:Software_Log rdf:type owl:Class ;
                            rdfs:subClassOf PSS-ontology-2:Product_Data ;
                            obo:IAO_0000115 "Digital Log Data are Product Data generated from a software element, part of the product." ;
                            dc:contributor "ATB - EPFL" ;
                            rdfs:label "Digital Log Data" .


###  http://www.semanticweb.org/atb/ontologies/2019/11/PSS-ontology-2#System
PSS-ontology-2:System rdf:type owl:Class ;
                      rdfs:subClassOf obo:BFO_0000020 ;
                      obo:IAO_0000115 "System is a regularly interacting or interdependent group of items forming a unified whole [14]. Every system is delineated by its spatial and temporal boundaries, surrounded and influenced by its environment, described by its structure and purpose and expressed in its functioning [13]. In engineering and physics, a physical system is the portion of the universe that is being studied (of which a thermodynamic system is one major example). Engineering also has the concept of a system that refers to all of the parts and interactions between parts of a complex project. Systems engineering refers to the branch of engineering that studies how this type of system should be planned, designed, implemented, built, and maintained. System is a set of interacting elements [6] that, as a unity, affects the design/development of solutions. It is considered from the approach of System Engineering." ;
                      obo:IAO_0000119 """Resources:

6. IEC, ISO. \"15288-2008. System engineering and software engineering–System life cycle processes.\" (2008), 
< https://www.iso.org/standard/43564.html> [accessed 20 July 2017]

13. Wikipedia contributors, 'System', Wikipedia, The Free Encyclopedia, 6 September 2017, 11:52 UTC, <https://en.wikipedia.org/w/index.php?title=System&oldid=799223483> [accessed 20 September 2017]

14.  \"Definition of system\". Merriam-Webster. Springfield, MA, USA. Retrieved 2016-10-09.""" ;
                      rdfs:comment "This is an interface class to other ontologies." ;
                      rdfs:label "system" .


###  http://www.semanticweb.org/atb/ontologies/2019/11/PSS-ontology-2#Stakeholder/Actor
<http://www.semanticweb.org/atb/ontologies/2019/11/PSS-ontology-2#Stakeholder/Actor> rdf:type owl:Class ;
                                                                                     rdfs:subClassOf obo:BFO_0000040 ;
                                                                                     obo:IAO_0000115 "Stakeholder/Actor is an entity that describes the humans (or beings) involved in a PSS (development, deployment, use etc.)." ;
                                                                                     dc:contributor "ATB - EPFL" ;
                                                                                     rdfs:comment "It may serve as an interface class for merging with other ontologies" ;
                                                                                     rdfs:label "Stakeholder/Actor" .


###  http://www.semanticweb.org/atb/ontologies/2019/11/PSS-ontology-2#Supplier/Provider/Vendor
<http://www.semanticweb.org/atb/ontologies/2019/11/PSS-ontology-2#Supplier/Provider/Vendor> rdf:type owl:Class ;
                                                                                            rdfs:subClassOf PSS-ontology-2:Company ;
                                                                                            obo:IAO_0000115 "Supplier/Provider/Vendor is a Company that both produces and sells something (product, service, PSS), or only sells it." ;
                                                                                            dc:contributor "ATB - EPFL" ;
                                                                                            rdfs:comment "Additional subclasses are possible, e.g. in DIVERSITY material supplier, component supplier etc." ;
                                                                                            rdfs:label "Supplier/Provider/Vendor" .


###  Generated by the OWL API (version 4.5.9.2019-02-01T07:24:44Z) https://github.com/owlcs/owlapi
